zoo_saturn/mpmc_bqueue: Rewrite.

theories/zoo_saturn/mpmc_bqueue.v
@@ -32,9 +32,9 @@ From zoo Require Import
   options.
 
 Implicit Types b : bool.
-Implicit Types l front node back new_back : location.
+Implicit Types front node back new_back : location.
 Implicit Types hist past nodes : list location.
-Implicit Types v t : val.
+Implicit Types v : val.
 Implicit Types vs : list val.
 Implicit Types waiter : gname.
 Implicit Types waiters : gmap gname nat.
@@ -80,170 +80,1290 @@ Proof.
   solve_inG.
 Qed.
 
+Module base.
+  Section mpmc_bqueue_G.
+    Context `{mpmc_bqueue_G : MpmcBqueueG Σ}.
+
+    Implicit Types t : location.
+
+    Record mpmc_bqueue_name := {
+      mpmc_bqueue_name_inv : namespace ;
+      mpmc_bqueue_name_capacity : nat ;
+      mpmc_bqueue_name_history : gname ;
+      mpmc_bqueue_name_front : gname ;
+      mpmc_bqueue_name_model : gname ;
+      mpmc_bqueue_name_waiters : gname ;
+    }.
+    Implicit Types γ : mpmc_bqueue_name.
+
+    #[global] Instance mpmc_bqueue_name_eq_dec : EqDecision mpmc_bqueue_name :=
+      ltac:(solve_decision).
+    #[global] Instance mpmc_bqueue_name_countable :
+      Countable mpmc_bqueue_name.
+    Proof.
+      solve_countable.
+    Qed.
+
+    #[local] Definition history_auth' γ_history :=
+      mono_list_auth γ_history (DfracOwn 1).
+    #[local] Definition history_auth γ :=
+      history_auth' γ.(mpmc_bqueue_name_history).
+    #[local] Definition history_at γ :=
+      mono_list_at γ.(mpmc_bqueue_name_history).
+
+    #[local] Definition front_auth' γ_front :=
+      auth_nat_max_auth γ_front (DfracOwn 1).
+    #[local] Definition front_auth γ :=
+      front_auth' γ.(mpmc_bqueue_name_front).
+    #[local] Definition front_lb γ :=
+      auth_nat_max_lb γ.(mpmc_bqueue_name_front).
+
+    #[local] Definition model₁' γ_model vs :=
+      twins_twin1 γ_model (DfracOwn 1) vs.
+    #[local] Definition model₁ γ :=
+      model₁' γ.(mpmc_bqueue_name_model).
+    #[local] Definition model₂' γ_model vs :=
+      twins_twin2 γ_model vs.
+    #[local] Definition model₂ γ :=
+      model₂' γ.(mpmc_bqueue_name_model).
+
+    #[local] Definition waiters_auth' γ_waiters :=
+      ghost_map_auth γ_waiters 1.
+    #[local] Definition waiters_auth γ :=
+      waiters_auth' γ.(mpmc_bqueue_name_waiters).
+    #[local] Definition waiters_at γ waiter :=
+      ghost_map_elem γ.(mpmc_bqueue_name_waiters) waiter (DfracOwn 1).
+
+    #[local] Definition node_model γ node (i : nat) b : iProp Σ :=
+      node ↦ₕ Header §Node 4 ∗
+      node.[index] ↦□ #i ∗
+      history_at γ i node ∗
+      if b then front_lb γ i else True%I.
+    #[local] Instance : CustomIpatFormat "node_model" :=
+      " ( #H{}_header &
+          #H{}_index &
+          #Hhistory_at_{} &
+          {{front}#Hfront_lb_{};_}
+        )
+      ".
+
+    #[local] Definition waiter_au γ (Ψ : bool → iProp Σ) : iProp Σ :=
+      AU <{
+        ∃∃ vs,
+        model₁ γ vs
+      }> @ ⊤ ∖ ↑γ.(mpmc_bqueue_name_inv), ∅ <{
+        model₁ γ vs
+      , COMM
+        Ψ (bool_decide (vs = []))
+      }>.
+    #[local] Definition waiter_model γ past waiter i : iProp Σ :=
+      ∃ Ψ,
+      saved_pred waiter Ψ ∗
+      if decide (i < length past) then
+        Ψ false
+      else
+        waiter_au γ Ψ.
+
+    #[local] Definition inv_inner t γ : iProp Σ :=
+      ∃ hist past front nodes back vs waiters,
+      ⌜hist = past ++ front :: nodes⌝ ∗
+      ⌜back ∈ hist⌝ ∗
+      t.[front] ↦ #front ∗
+      t.[back] ↦ #back ∗
+      xtchain (Header §Node 4) (DfracOwn 1) hist §Null ∗
+      ( [∗ list] node; v ∈ nodes; vs,
+        node.[data] ↦ v
+      ) ∗
+      ( [∗ list] i ↦ node ∈ hist,
+        node.[index] ↦□ #i
+      ) ∗
+      ( [∗ list] i ↦ node ∈ hist,
+        ∃ cap : nat,
+        node.[estimated_capacity] ↦ #cap ∗
+        ⌜i + cap ≤ length past + γ.(mpmc_bqueue_name_capacity)⌝
+      ) ∗
+      history_auth γ hist ∗
+      front_auth γ (length past) ∗
+      model₂ γ vs ∗
+      waiters_auth γ waiters ∗
+      ( [∗ map] waiter ↦ i ∈ waiters,
+        waiter_model γ past waiter i
+      ).
+    #[local] Instance : CustomIpatFormat "inv_inner" :=
+      " ( %hist{} &
+          %past{} &
+          %front{} &
+          %nodes{} &
+          %back{} &
+          %vs{} &
+          %waiters{} &
+          >%Hhist{} &
+          >%Hback{} &
+          >Ht_front &
+          >Ht_back &
+          >Hhist &
+          >Hnodes &
+          >Hindices &
+          >Hcapacities &
+          >Hhistory_auth &
+          >Hfront_auth &
+          >Hmodel₂ &
+          >Hwaiters_auth &
+          Hwaiters
+        )
+      ".
+    #[local] Definition inv' t γ :=
+      inv γ.(mpmc_bqueue_name_inv) (inv_inner t γ).
+    Definition mpmc_bqueue_inv t γ ι cap : iProp Σ :=
+      ⌜ι = γ.(mpmc_bqueue_name_inv)⌝ ∗
+      ⌜cap = γ.(mpmc_bqueue_name_capacity)⌝ ∗
+      t.[capacity] ↦□ #cap ∗
+      inv' t γ.
+    #[local] Instance : CustomIpatFormat "inv" :=
+      " ( -> &
+          -> &
+          #Ht_capacity &
+          #Hinv
+        )
+      ".
+
+    Definition mpmc_bqueue_model γ vs : iProp Σ :=
+      ⌜length vs ≤ γ.(mpmc_bqueue_name_capacity)⌝ ∗
+      model₁ γ vs.
+    #[local] Instance : CustomIpatFormat "model" :=
+      " ( % &
+          Hmodel₁{_{}}
+        )
+      ".
+
+    #[global] Instance mpmc_bqueue_model_timeless γ vs :
+      Timeless (mpmc_bqueue_model γ vs).
+    Proof.
+      apply _.
+    Qed.
+
+    #[global] Instance mpmc_bqueue_inv_persistent t γ ι cap :
+      Persistent (mpmc_bqueue_inv t γ ι cap).
+    Proof.
+      apply _.
+    Qed.
+
+    #[local] Lemma history_alloc front :
+      ⊢ |==>
+        ∃ γ_history,
+        history_auth' γ_history [front].
+    Proof.
+      apply mono_list_alloc.
+    Qed.
+    #[local] Lemma history_at_get {γ hist} i node :
+      hist !! i = Some node →
+      history_auth γ hist ⊢
+      history_at γ i node.
+    Proof.
+      apply mono_list_at_get.
+    Qed.
+    #[local] Lemma history_at_agree γ i node1 node2 :
+      history_at γ i node1 -∗
+      history_at γ i node2 -∗
+      ⌜node1 = node2⌝.
+    Proof.
+      apply mono_list_at_agree.
+    Qed.
+    #[local] Lemma history_at_lookup γ hist i node :
+      history_auth γ hist -∗
+      history_at γ i node -∗
+      ⌜hist !! i = Some node⌝.
+    Proof.
+      apply mono_list_at_valid.
+    Qed.
+    #[local] Lemma history_at_elem_of γ hist i node :
+      history_auth γ hist -∗
+      history_at γ i node -∗
+      ⌜node ∈ hist⌝.
+    Proof.
+      iIntros "Hauth Hat".
+      iDestruct (history_at_lookup with "Hauth Hat") as %?%list_elem_of_lookup_2.
+      iSteps.
+    Qed.
+    #[local] Lemma history_update {γ hist} node :
+      history_auth γ hist ⊢ |==>
+        history_auth γ (hist ++ [node]) ∗
+        history_at γ (length hist) node.
+    Proof.
+      iIntros "Hauth".
+      iMod (mono_list_update_snoc with "Hauth") as "Hauth".
+      iDestruct (history_at_get with "Hauth") as "#Hat".
+      { rewrite lookup_snoc_Some. naive_solver. }
+      iSteps.
+    Qed.
+
+    #[local] Lemma front_alloc :
+      ⊢ |==>
+        ∃ γ_front,
+        front_auth' γ_front 0.
+    Proof.
+      apply auth_nat_max_alloc.
+    Qed.
+    #[local] Lemma front_lb_get γ i :
+      front_auth γ i ⊢
+      front_lb γ i.
+    Proof.
+      apply auth_nat_max_lb_get.
+    Qed.
+    #[local] Lemma front_lb_valid γ i1 i2 :
+      front_auth γ i1 -∗
+      front_lb γ i2 -∗
+      ⌜i2 ≤ i1⌝.
+    Proof.
+      apply auth_nat_max_lb_valid.
+    Qed.
+    #[local] Lemma front_update {γ i} i' :
+      i ≤ i' →
+      front_auth γ i ⊢ |==>
+      front_auth γ i'.
+    Proof.
+      apply auth_nat_max_update.
+    Qed.
+
+    #[local] Lemma model_alloc :
+      ⊢ |==>
+        ∃ γ_model,
+        model₁' γ_model [] ∗
+        model₂' γ_model [].
+    Proof.
+      apply twins_alloc'.
+    Qed.
+    #[local] Lemma model₁_exclusive γ vs1 vs2 :
+      model₁ γ vs1 -∗
+      model₁ γ vs2 -∗
+      False.
+    Proof.
+      apply twins_twin1_exclusive.
+    Qed.
+    #[local] Lemma model_agree γ vs1 vs2 :
+      model₁ γ vs1 -∗
+      model₂ γ vs2 -∗
+      ⌜vs1 = vs2⌝.
+    Proof.
+      apply: twins_agree_L.
+    Qed.
+    #[local] Lemma model_update {γ vs1 vs2} vs :
+      model₁ γ vs1 -∗
+      model₂ γ vs2 ==∗
+        model₁ γ vs ∗
+        model₂ γ vs.
+    Proof.
+      apply twins_update.
+    Qed.
+
+    #[local] Lemma waiters_alloc :
+      ⊢ |==>
+        ∃ γ_waiters,
+        waiters_auth' γ_waiters ∅.
+    Proof.
+      iMod ghost_map_alloc as "(%γ_waiters & Hwaiters_auth & _)".
+      iSteps.
+    Qed.
+    #[local] Lemma waiters_insert {γ waiters} i Ψ :
+      waiters_auth γ waiters ⊢ |==>
+        ∃ waiter,
+        waiters_auth γ (<[waiter := i]> waiters) ∗
+        saved_pred waiter Ψ ∗
+        waiters_at γ waiter i.
+    Proof.
+      iIntros "Hwaiters_auth".
+      iMod (saved_pred_alloc_cofinite (dom waiters) Ψ) as "(%waiter & %Hwaiter & $)".
+      rewrite not_elem_of_dom in Hwaiter.
+      iApply (ghost_map_insert with "Hwaiters_auth"); first done.
+    Qed.
+    #[local] Lemma waiters_delete γ waiters waiter i :
+      waiters_auth γ waiters -∗
+      waiters_at γ waiter i ==∗
+        ⌜waiters !! waiter = Some i⌝ ∗
+        waiters_auth γ (delete waiter waiters).
+    Proof.
+      iIntros "Hwaiters_auth Hwaiters_at".
+      iDestruct (ghost_map_lookup with "Hwaiters_auth Hwaiters_at") as %?.
+      iMod (ghost_map_delete with "Hwaiters_auth Hwaiters_at") as "$".
+      iSteps.
+    Qed.
+
+    Lemma mpmc_bqueue_model_valid t γ ι cap vs :
+      mpmc_bqueue_inv t γ ι cap -∗
+      mpmc_bqueue_model γ vs -∗
+      ⌜length vs ≤ cap⌝.
+    Proof.
+      iSteps.
+    Qed.
+    Lemma mpmc_bqueue_model_exclusive γ vs1 vs2 :
+      mpmc_bqueue_model γ vs1 -∗
+      mpmc_bqueue_model γ vs2 -∗
+      False.
+    Proof.
+      iIntros "(:model =1) (:model =2)".
+      iApply (model₁_exclusive with "Hmodel₁_1 Hmodel₁_2").
+    Qed.
+
+    Lemma mpmc_bqueue_create_spec ι cap :
+      (0 ≤ cap)%Z →
+      {{{
+        True
+      }}}
+        mpmc_bqueue_create #cap
+      {{{ t γ,
+        RET #t;
+        meta_token t ⊤ ∗
+        mpmc_bqueue_inv t γ ι ₊cap ∗
+        mpmc_bqueue_model γ []
+      }}}.
+    Proof.
+      iIntros "%Hcap %Φ _ HΦ".
+
+      wp_rec.
+      wp_block front as "Hfront_header" "_" "(Hfront_next & Hfront_data & Hfront_index & Hfront_capacity & _)".
+      iMod (pointsto_persist with "Hfront_index") as "#Hfront_index".
+      wp_block t as "Hmeta" "(Ht_capacity & Ht_front & Ht_back & _)".
+      iMod (pointsto_persist with "Ht_capacity") as "#Hcapacity".
+
+      iMod history_alloc as "(%γ_history & Hhistory_auth)".
+      iMod front_alloc as "(%γ_front & Hfront_auth)".
+      iMod model_alloc as "(%γ_model & Hmodel₁ & Hmodel₂)".
+      iMod waiters_alloc as "(%γ_waiters & Hwaiters_auth)".
+
+      pose γ := {|
+        mpmc_bqueue_name_inv := ι ;
+        mpmc_bqueue_name_capacity := ₊cap ;
+        mpmc_bqueue_name_history := γ_history ;
+        mpmc_bqueue_name_front := γ_front ;
+        mpmc_bqueue_name_model := γ_model ;
+        mpmc_bqueue_name_waiters := γ_waiters ;
+      |}.
+
+      iApply ("HΦ" $! t γ).
+      iFrame. iSplitL; last iSteps.
+      iStep 3.
+      iApply inv_alloc.
+      iExists [front], [], front, [], front, [], ∅. iFrameSteps.
+      - rewrite list_elem_of_singleton //.
+      - rewrite xtchain_singleton big_sepM_empty. iSteps.
+    Qed.
+
+    Lemma mpmc_bqueue_capacity_spec t γ ι cap :
+      {{{
+        mpmc_bqueue_inv t γ ι cap
+      }}}
+        mpmc_bqueue_capacity #t
+      {{{
+        RET #cap;
+        True
+      }}}.
+    Proof.
+      iSteps.
+    Qed.
+
+    #[local] Lemma front_spec_strong Ψ t γ :
+      {{{
+        inv' t γ ∗
+        if Ψ is Some Ψ then
+          waiter_au γ Ψ
+        else
+          True
+      }}}
+        (#t).{front}
+      {{{ front i,
+        RET #front;
+        node_model γ front i true ∗
+        if Ψ is Some Ψ then
+          ∃ waiter,
+          saved_pred waiter Ψ ∗
+          waiters_at γ waiter i
+        else
+          True
+      }}}.
+    Proof.
+      iIntros "%Φ (#Hinv & HΨ) HΦ".
+
+      iInv "Hinv" as "(:inv_inner)".
+      wp_load.
+      assert (hist !! (length past) = Some front) as Hlookup.
+      { rewrite Hhist list_lookup_middle //. }
+      iDestruct (xtchain_lookup_header with "Hhist") as "#Hfront_header"; first done.
+      iDestruct (big_sepL_lookup with "Hindices") as "#Hfront_index"; first done.
+      iDestruct (history_at_get _ front with "Hhistory_auth") as "#Hhistory_at_front"; first done.
+      iDestruct (front_lb_get with "Hfront_auth") as "#Hfront_lb_front".
+      destruct Ψ as [Ψ |]; last iSteps.
+      iMod (waiters_insert (length past) Ψ with "Hwaiters_auth") as "(%waiter & Hwaiter_auth & #Hwaiter & Hwaiters_at)".
+      iDestruct (big_sepM_insert_2 _ _ waiter (length past) with "[HΨ] Hwaiters") as "Hwaiters".
+      { iExists Ψ. rewrite decide_False; first lia. iSteps. }
+      iSplitR "Hwaiters_at HΦ". { iFrameSteps. }
+      iSteps.
+    Qed.
+    #[local] Lemma front_spec t γ :
+      {{{
+        inv' t γ
+      }}}
+        (#t).{front}
+      {{{ front i,
+        RET #front;
+        node_model γ front i true
+      }}}.
+    Proof.
+      iIntros "%Φ #Hinv HΦ".
+      wp_apply (front_spec_strong None with "[$Hinv]").
+      iSteps.
+    Qed.
+
+    #[local] Lemma back_spec t γ :
+      {{{
+        inv' t γ
+      }}}
+        (#t).{back}
+      {{{ back i,
+        RET #back;
+        node_model γ back i false
+      }}}.
+    Proof.
+      iIntros "%Φ #Hinv HΦ".
+
+      iInv "Hinv" as "(:inv_inner)".
+      wp_load.
+      pose proof Hback as (i & Hlookup)%list_elem_of_lookup.
+      iDestruct (xtchain_lookup_header with "Hhist") as "#Hback_header"; first done.
+      iDestruct (big_sepL_lookup with "Hindices") as "#Hback_index"; first done.
+      iDestruct (history_at_get with "Hhistory_auth") as "#Hhistory_at_back"; first done.
+      iSplitR "HΦ". { iFrameSteps. }
+      iSteps.
+    Qed.
+
+    Inductive operation :=
+      | Size (i_front : nat) (Ψ : val → iProp Σ)
+      | IsEmpty waiter (Ψ : bool → iProp Σ)
+      | Pop (Ψ : option val → iProp Σ)
+      | Other.
+    Implicit Types op : operation.
+    Inductive operation' :=
+      | Size'
+      | IsEmpty'
+      | Pop'
+      | Other'.
+    #[local] Instance operation'_eq_dec : EqDecision operation' :=
+      ltac:(solve_decision).
+    #[local] Coercion operation_to_operation' op :=
+      match op with
+      | Size _ _ =>
+          Size'
+      | IsEmpty _ _ =>
+          IsEmpty'
+      | Pop _ =>
+          Pop'
+      | Other =>
+          Other'
+      end.
+    #[local] Definition size_au γ Ψ : iProp Σ :=
+      AU <{
+        ∃∃ vs,
+        mpmc_bqueue_model γ vs
+      }> @ ⊤ ∖ ↑γ.(mpmc_bqueue_name_inv), ∅ <{
+        mpmc_bqueue_model γ vs
+      , COMM
+        True -∗ Ψ #(length vs)
+      }>.
+    #[local] Definition pop_au γ (Ψ : option val → iProp Σ) : iProp Σ :=
+      AU <{
+        ∃∃ vs,
+        model₁ γ vs
+      }> @ ⊤ ∖ ↑γ.(mpmc_bqueue_name_inv), ∅ <{
+        model₁ γ (tail vs)
+      , COMM
+        True -∗ Ψ (head vs)
+      }>.
+    #[local] Lemma next_spec_aux (next : option location) op t γ i node :
+      {{{
+        inv' t γ ∗
+        history_at γ i node ∗
+        from_option (history_at γ (S i)) True next ∗
+        match op with
+        | Size i_front Ψ =>
+            front_lb γ i_front ∗
+            size_au γ Ψ
+        | IsEmpty waiter Ψ =>
+            front_lb γ i ∗
+            saved_pred waiter Ψ ∗
+            waiters_at γ waiter i ∗
+            £ 1
+        | Pop Ψ =>
+            front_lb γ i ∗
+            pop_au γ Ψ
+        | Other =>
+            True
+        end
+      }}}
+        (#node).{next}
+      {{{ res,
+        RET res;
+          ⌜res = §Null%V⌝ ∗
+          from_option (const False) True next ∗
+          match op with
+          | Size i_front Ψ =>
+                Ψ #(i - i_front)
+              ∨ ∃ i_front',
+                front_lb γ i_front' ∗
+                ⌜i_front < i_front'⌝ ∗
+                size_au γ Ψ
+          | IsEmpty waiter Ψ =>
+              Ψ true
+          | Pop Ψ =>
+              Ψ None
+          | _ =>
+              True
+          end
+       ∨ ∃ node',
+          ⌜res = #node'⌝ ∗
+          node_model γ node' (S i) false ∗
+          ⌜from_option (node' =.) True next⌝ ∗
+          match op with
+          | Size _ Ψ =>
+              size_au γ Ψ
+          | IsEmpty waiter Ψ =>
+              Ψ false
+          | Pop Ψ =>
+              pop_au γ Ψ
+          | Other =>
+              True
+          end
+      }}}.
+    Proof.
+      iIntros "%Φ (#Hinv & #Hhistory_at_node & #Hhistory_at_next & Hop) HΦ".
+
+      iInv "Hinv" as "(:inv_inner)".
+      iDestruct (history_at_lookup with "Hhistory_auth Hhistory_at_node") as %Hlookup.
+      iDestruct (xtchain_lookup_acc with "Hhist") as "(_ & Hnode & Hhist)"; first done.
+      wp_load.
+      iDestruct ("Hhist" with "Hnode") as "Hhist".
+      destruct (hist !! S i) as [node' |] eqn:Hlookup'; simpl.
+
+      - iDestruct (xtchain_lookup_header with "Hhist") as "#Hnode'_header"; first done.
+        iDestruct (big_sepL_lookup with "Hindices") as "#Hnode'_index"; first done.
+        iDestruct (history_at_get (S i) with "Hhistory_auth") as "#Hhistory_at_node'"; first done.
+
+        iAssert ⌜from_option (node' =.) True next⌝%I as %?.
+        { destruct next as [next |]; last done.
+          iApply (history_at_agree with "Hhistory_at_node' Hhistory_at_next").
+        }
+
+        destruct op. 1,3,4: iSteps.
+        iDestruct "Hop" as "(#Hfront_lb_node & #Hwaiter & Hwaiters_at & H£)".
+        iMod (waiters_delete with "Hwaiters_auth Hwaiters_at") as "(%Hwaiters_lookup & Hwaiters_auth)".
+        iDestruct (big_sepM_delete with "Hwaiters") as "((%Ψ_ & Hwaiter_ & HΨ) & Hwaiters)"; first done.
+        iDestruct (saved_pred_agree false with "Hwaiter Hwaiter_") as "Heq".
+        iMod (lc_fupd_elim_later with "H£ Heq") as "Heq".
+        destruct_decide (i = length past) as -> | Hi.
+
+        + rewrite decide_False; first lia.
+
+          iMod "HΨ" as "(%vs_ & Hmodel₁ & _ & HΨ)".
+          iDestruct (model_agree with "Hmodel₁ Hmodel₂") as %->.
+          iMod ("HΨ" with "Hmodel₁") as "HΨ".
+          assert (nodes ≠ []) as Hnodes.
+          { apply lookup_lt_Some in Hlookup'.
+            rewrite Hhist length_app /= in Hlookup'.
+            naive_solver lia.
+          }
+          iAssert ⌜vs ≠ []⌝%I as %Hvs.
+          { destruct_decide (vs = []) as -> | ?; last done.
+            iDestruct (big_sepL2_length with "Hnodes") as %->%nil_length_inv.
+            iSteps.
+          }
+          rewrite bool_decide_eq_false_2 //.
+
+          iSplitR "Heq HΨ HΦ". { iFrameSteps. }
+          iSteps. iRewrite "Heq". iSteps.
+
+        + iDestruct (front_lb_valid with "Hfront_auth Hfront_lb_node") as %Hi_.
+          rewrite decide_True; first lia.
+          iSplitR "Heq HΨ HΦ". { iFrameSteps. }
+          iSteps. iRewrite "Heq". iSteps.
+
+      - destruct next as [next |].
+        { iDestruct (history_at_lookup with "Hhistory_auth Hhistory_at_next") as %?. congruence. }
+
+        destruct op as [i_front | | |].
+
+        + iDestruct "Hop" as "(#Hfront_lb_front & HΨ)".
+          destruct_decide (length past = i_front).
+
+          * iMod "HΨ" as "(%vs_ & (:model) & _ & HΨ)".
+            iDestruct (model_agree with "Hmodel₁ Hmodel₂") as %->.
+            iMod ("HΨ" with "[$Hmodel₁ //] [//]") as "HΨ".
+            assert ((i - i_front)%Z = length nodes) as ->.
+            { opose proof* length_lookup_last as Hlength; [done.. |].
+              rewrite Hhist length_app /= in Hlength.
+              lia.
+            }
+            iDestruct (big_sepL2_length with "Hnodes") as %->.
+
+            iSplitR "HΨ HΦ". { iFrameSteps. }
+            iSteps.
+
+          * iDestruct (front_lb_valid with "Hfront_auth Hfront_lb_front") as %?. iClear "Hfront_lb_front".
+            iDestruct (front_lb_get with "Hfront_auth") as "#Hfront_lb_front".
+            iSplitR "HΨ HΦ". { iFrameSteps. }
+            iSteps.
+
+        + iDestruct "Hop" as "(#Hfront_lb_node & #Hwaiter & Hwaiters_at & H£)".
+          iDestruct (front_lb_valid with "Hfront_auth Hfront_lb_node") as %Hi.
+          opose proof* length_lookup_last as Hlength; [done.. |].
+          rewrite Hhist length_app /= in Hlength.
+          assert (i = length past) as -> by lia.
+          assert (length nodes = 0) as ->%nil_length_inv by lia.
+          iDestruct (big_sepL2_length with "Hnodes") as %->%symmetry%nil_length_inv.
+          iMod (waiters_delete with "Hwaiters_auth Hwaiters_at") as "(%Hwaiters_lookup & Hwaiters_auth)".
+          iDestruct (big_sepM_delete with "Hwaiters") as "((%Ψ_ & Hwaiter_ & HΨ) & Hwaiters)"; first done.
+          iDestruct (saved_pred_agree true with "Hwaiter Hwaiter_") as "Heq".
+          iMod (lc_fupd_elim_later with "H£ Heq") as "Heq".
+          rewrite decide_False; first lia.
+
+          iMod "HΨ" as "(%vs & Hmodel₁ & _ & HΨ)".
+          iDestruct (model_agree with "Hmodel₁ Hmodel₂") as %->.
+          iMod ("HΨ" with "Hmodel₁") as "HΨ".
+
+          iSplitR "Heq HΨ HΦ". { iFrameSteps. }
+          iIntros "!> {%}".
+
+          iApply "HΦ".
+          iLeft. iRewrite "Heq". iSteps.
+
+        + iDestruct "Hop" as "(#Hfront_lb_node & HΨ)".
+          iDestruct (front_lb_valid with "Hfront_auth Hfront_lb_node") as %Hi.
+          opose proof* length_lookup_last as Hlength; [done.. |].
+          rewrite Hhist length_app /= in Hlength.
+          assert (i = length past) as -> by lia.
+          assert (length nodes = 0) as ->%nil_length_inv by lia.
+          iDestruct (big_sepL2_length with "Hnodes") as %->%symmetry%nil_length_inv.
+
+          iMod "HΨ" as "(%vs & Hmodel₁ & _ & HΨ)".
+          iDestruct (model_agree with "Hmodel₁ Hmodel₂") as %->.
+          iMod ("HΨ" with "Hmodel₁") as "HΨ".
+
+          iSplitR "HΨ HΦ". { iFrameSteps. }
+          iSteps.
+
+        + iSteps.
+    Qed.
+    #[local] Lemma next_spec {t γ i} node :
+      {{{
+        inv' t γ ∗
+        history_at γ i node
+      }}}
+        (#node).{next}
+      {{{ res,
+        RET res;
+          ⌜res = §Null%V⌝
+        ∨ ∃ node',
+          ⌜res = #node'⌝ ∗
+          node_model γ node' (S i) false
+      }}}.
+    Proof.
+      iIntros "%Φ (#Hinv & #Hhistory_at_node) HΦ".
+      wp_apply (next_spec_aux None Other); iSteps.
+    Qed.
+    #[local] Lemma next_spec' {t γ i} node next :
+      {{{
+        inv' t γ ∗
+        history_at γ i node ∗
+        history_at γ (S i) next
+      }}}
+        (#node).{next}
+      {{{
+        RET #next;
+        node_model γ next (S i) false
+      }}}.
+    Proof.
+      iIntros "%Φ (#Hinv & #Hhistory_at_node & #Hhistory_at_next) HΦ".
+      wp_apply (next_spec_aux (Some next) Other); iSteps.
+    Qed.
+    #[local] Lemma next_spec_size {t γ i node} i_front Ψ :
+      {{{
+        inv' t γ ∗
+        history_at γ i node ∗
+        front_lb γ i_front ∗
+        size_au γ Ψ
+      }}}
+        (#node).{next}
+      {{{ res,
+        RET res;
+          ⌜res = §Null%V⌝ ∗
+          ( Ψ #(i - i_front)
+          ∨ ∃ i_front',
+            front_lb γ i_front' ∗
+            ⌜i_front < i_front'⌝ ∗
+            size_au γ Ψ
+          )
+       ∨ ∃ node',
+          ⌜res = #node'⌝ ∗
+          node_model γ node' (S i) false ∗
+          size_au γ Ψ
+      }}}.
+    Proof.
+      iIntros "%Φ (#Hinv & #Hhistory_at_node & #Hfront_lb_front & HΨ) HΦ".
+      wp_apply (next_spec_aux None (Size _ _) with "[$]").
+      iSteps.
+    Qed.
+    #[local] Lemma next_spec_is_empty {t γ i node} waiter Ψ :
+      {{{
+        inv' t γ ∗
+        history_at γ i node ∗
+        front_lb γ i ∗
+        saved_pred waiter Ψ ∗
+        waiters_at γ waiter i ∗
+        £ 1
+      }}}
+        (#node).{next}
+      {{{ res,
+        RET res;
+          ⌜res = §Null%V⌝ ∗
+          Ψ true
+        ∨ ∃ node',
+          ⌜res = #node'⌝ ∗
+          node_model γ node' (S i) false ∗
+          Ψ false
+      }}}.
+    Proof.
+      iIntros "%Φ (#Hinv & #Hhistory_at_node & #Hfront_lb_node & #Hwaiter & Hwaiters_at & H£) HΦ".
+      wp_apply (next_spec_aux None (IsEmpty _ _) with "[$]").
+      iSteps.
+    Qed.
+    #[local] Lemma next_spec_pop {t γ i node} Ψ :
+      {{{
+        inv' t γ ∗
+        history_at γ i node ∗
+        front_lb γ i ∗
+        pop_au γ Ψ
+      }}}
+        (#node).{next}
+      {{{ res,
+        RET res;
+          ⌜res = §Null%V⌝ ∗
+          Ψ None
+        ∨ ∃ node',
+          ⌜res = #node'⌝ ∗
+          node_model γ node' (S i) false ∗
+          pop_au γ Ψ
+      }}}.
+    Proof.
+      iIntros "%Φ (#Hinv & #Hhistory_at_node & #Hfront_lb_node & HΨ) HΦ".
+      wp_apply (next_spec_aux None (Pop _) with "[$]").
+      iSteps.
+    Qed.
+
+    Lemma mpmc_bqueue_size_spec t γ ι cap :
+      <<<
+        mpmc_bqueue_inv t γ ι cap
+      | ∀∀ vs,
+        mpmc_bqueue_model γ vs
+      >>>
+        mpmc_bqueue_size #t @ ↑ι
+      <<<
+        mpmc_bqueue_model γ vs
+      | RET #(length vs);
+        True
+      >>>.
+    Proof.
+      iIntros "%Φ (:inv) HΦ".
+
+      iLöb as "HLöb".
+
+      wp_rec.
+      wp_apply (front_spec with "Hinv") as (front1 i_front1) "(:node_model =front1 front=)".
+      wp_match.
+      wp_smart_apply (prophet_typed_strong_1_wp_proph prophet with "[//]") as (pid proph) "Hproph".
+      wp_smart_apply (back_spec with "Hinv") as (back2 i_back2) "(:node_model =back2)".
+      wp_match. wp_pures.
+      destruct_decide (proph = front1) as -> | Hproph.
+
+      - wp_apply (next_spec_size with "[$]") as (res) "[(-> & HΦ) | (%node & -> & (:node_model =node) & HΦ)]".
+
+        + wp_pures.
+
+          wp_bind (Resolve _ _ _).
+          iInv "Hinv" as "(:inv_inner =3)".
+          wp_apply (prophet_typed_strong_1_wp_resolve with "Hproph"); first done.
+          wp_load.
+          iStep. iIntros "<-".
+          iDestruct "HΦ" as "[HΦ | (%i_front2 & #Hfront_lb_front2 & % & HΦ)]"; last first.
+          { assert (hist3 !! (length past3) = Some front1) as Hlookup.
+            { rewrite Hhist3 list_lookup_middle //. }
+            iDestruct (big_sepL_lookup with "Hindices") as "#Hfront1_index_"; first done.
+            iDestruct (pointsto_agree with "Hfront1_index Hfront1_index_") as %[= ?%(inj _)].
+            iDestruct (front_lb_valid with "Hfront_auth Hfront_lb_front2") as %?.
+            lia.
+          }
+          iSteps.
+
+        + wp_match. wp_pures.
+
+          wp_bind (CAS _ _ _).
+          iInv "Hinv" as "(:inv_inner =3)".
+          wp_apply (wp_cas_nobranch' with "Ht_back") as (b) "% Ht_back".
+          iSplitR "HΦ".
+          { iDestruct (history_at_elem_of with "Hhistory_auth Hhistory_at_node") as %Hnode.
+            destruct b; iFrameSteps.
+          }
+          iSteps.
+
+      - wp_apply (next_spec with "[$]") as (res) "[-> | (%node & -> & (:node_model =node))]".
+
+        + wp_pures.
+
+          wp_bind (Resolve _ _ _).
+          iInv "Hinv" as "(:inv_inner =3)".
+          wp_apply (prophet_typed_strong_1_wp_resolve with "Hproph"); first done.
+          iSteps.
+
+        + wp_match. wp_pures.
+
+          wp_bind (CAS _ _ _).
+          iInv "Hinv" as "(:inv_inner =3)".
+          wp_apply (wp_cas_nobranch' with "Ht_back") as (b) "% Ht_back".
+          iSplitR "HΦ".
+          { iDestruct (history_at_elem_of with "Hhistory_auth Hhistory_at_node") as %Hnode.
+            destruct b; iFrameSteps.
+          }
+          iSteps.
+    Qed.
+
+    Lemma mpmc_bqueue_is_empty_spec t γ ι cap :
+      <<<
+        mpmc_bqueue_inv t γ ι cap
+      | ∀∀ vs,
+        mpmc_bqueue_model γ vs
+      >>>
+        mpmc_bqueue_is_empty #t @ ↑ι
+      <<<
+        mpmc_bqueue_model γ vs
+      | RET #(bool_decide (vs = []%list));
+        True
+      >>>.
+    Proof.
+      iIntros "%Φ (:inv) HΦ".
+
+      wp_rec credit:"H£".
+      wp_smart_apply (front_spec_strong (Some $ λ b, Φ #b) with "[$Hinv HΦ]") as (node i) "((:node_model =node front=) & %waiter & #Hwaiter & Hwaiters_at)".
+      { rewrite /= /waiter_au. iAuIntro.
+        iApply (aacc_aupd_commit with "HΦ"); first done. iIntros "%vs (:model)".
+        iAaccIntro with "Hmodel₁"; iSteps.
+      }
+      wp_match.
+      wp_smart_apply (next_spec_is_empty with "[$]"); iSteps.
+    Qed.
+
+    #[local] Lemma mpmc_bqueue_fix_back_spec {t γ} i {back} j new_back :
+      {{{
+        inv' t γ ∗
+        history_at γ i back ∗
+        node_model γ new_back j false
+      }}}
+        mpmc_bqueue_fix_back #t #back #new_back
+      {{{
+        RET ();
+        True
+      }}}.
+    Proof.
+      iIntros "%Φ (#Hinv & #Hhistory_at_back & (:node_model =new_back)) HΦ".
+
+      iLöb as "HLöb" forall (i back) "Hhistory_at_back".
+
+      wp_rec. wp_match.
+
+      wp_bind (_ and _)%E.
+      wp_apply (wp_wand itype_bool) as (res) "(%b & ->)".
+      { wp_smart_apply (next_spec new_back with "[$]") as (res) "[-> | (%new_back' & -> & (:node_model =new_back'))]"; last iSteps.
+        wp_pures.
+
+        wp_bind (CAS _ _ _).
+        iInv "Hinv" as "(:inv_inner =1)".
+        wp_cas as _ | [= ->]; first iSteps.
+        iDestruct (history_at_lookup with "Hhistory_auth Hhistory_at_new_back") as %Hnew_back%list_elem_of_lookup_2.
+        iSteps.
+      }
+
+      destruct b; last iSteps.
+      wp_smart_apply domain_yield_spec.
+      wp_smart_apply (back_spec with "Hinv") as (back' i') "(:node_model =back')".
+      iApply ("HLöb" with "HΦ Hhistory_at_back'").
+    Qed.
+
+    #[local] Lemma mpmc_bqueue_push_1_push_2_spec t γ new_back v :
+      ⊢ (
+        ∀ back i_back i_front (cap : Z),
+        <<<
+          t.[capacity] ↦□ #γ.(mpmc_bqueue_name_capacity) ∗
+          inv' t γ ∗
+          node_model γ back i_back false ∗
+          front_lb γ i_front ∗
+          ⌜0 ≤ cap⌝%Z ∗
+          ⌜i_back + cap ≤ i_front + γ.(mpmc_bqueue_name_capacity)⌝%Z ∗
+          new_back ↦ₕ Header §Node 4 ∗
+          new_back.[next] ↦ §Null ∗
+          new_back.[data] ↦ v ∗
+          new_back.[index] ↦- ∗
+          new_back.[estimated_capacity] ↦-
+        | ∀∀ vs,
+          ⌜length vs ≤ γ.(mpmc_bqueue_name_capacity)⌝ ∗
+          model₁ γ vs
+        >>>
+          mpmc_bqueue_push_1 #t #back #cap #new_back @ ↑γ.(mpmc_bqueue_name_inv)
+        <<<
+          ∃∃ b,
+          ⌜b = bool_decide (length vs < γ.(mpmc_bqueue_name_capacity))⌝ ∗
+          model₁ γ (if b then vs ++ [v] else vs)
+        | RET #b;
+          True
+        >>>
+      ) ∧ (
+        ∀ back i_back,
+        <<<
+          t.[capacity] ↦□ #γ.(mpmc_bqueue_name_capacity) ∗
+          inv' t γ ∗
+          node_model γ back i_back false ∗
+          new_back ↦ₕ Header §Node 4 ∗
+          new_back.[next] ↦ §Null ∗
+          new_back.[data] ↦ v ∗
+          new_back.[index] ↦- ∗
+          new_back.[estimated_capacity] ↦-
+        | ∀∀ vs,
+          ⌜length vs ≤ γ.(mpmc_bqueue_name_capacity)⌝ ∗
+          model₁ γ vs
+        >>>
+          mpmc_bqueue_push_2 #t #back #new_back @ ↑γ.(mpmc_bqueue_name_inv)
+        <<<
+          ∃∃ b,
+          ⌜b = bool_decide (length vs < γ.(mpmc_bqueue_name_capacity))⌝ ∗
+          model₁ γ (if b then vs ++ [v] else vs)
+        | RET #b;
+          True
+        >>>
+      ).
+    Proof.
+      iLöb as "HLöb".
+      iDestruct "HLöb" as "(IHpush_1 & IHpush_2)".
+      iSplit.
+
+      { iIntros "%back %i_back %i_front %cap %Φ (#Ht_capacity & #Hinv & (:node_model =back) & #Hfront_lb_front & % & % & #Hnew_back_header & Hnew_back_next & Hnew_back_data & (% & Hnew_back_index) & (% & Hnew_back_estimated_capacity)) HΦ".
+
+        wp_rec. do 2 wp_match. wp_pures.
+        case_bool_decide; wp_pures.
+
+        - wp_bind (_.{front})%E.
+          iInv "Hinv" as "(:inv_inner =1)".
+          wp_load.
+          assert (hist1 !! (length past1) = Some front1) as Hlookup.
+          { rewrite Hhist1 list_lookup_middle //. }
+          iDestruct (xtchain_lookup_header with "Hhist") as "#Hfront1_header"; first done.
+          iDestruct (big_sepL_lookup with "Hindices") as "#Hfront1_index"; first done.
+
+          destruct_decide (i_back < length past1 + γ.(mpmc_bqueue_name_capacity)) as Hnotfull | Hfull.
+
+          + iDestruct (front_lb_get with "Hfront_auth") as "#Hfront_lb_front1".
+            iSplitR "Hnew_back_next Hnew_back_data Hnew_back_index Hnew_back_estimated_capacity HΦ". { iFrameSteps. }
+            remember (length past1) as i_front1.
+            iModIntro. clear- Hnotfull.
+
+            wp_match. do 3 wp_load. wp_pures.
+            rewrite bool_decide_eq_false_2; first lia.
+            wp_pures.
+
+            wp_bind (_ <-{estimated_capacity} _)%E.
+            iInv "Hinv" as "(:inv_inner =2)".
+            iDestruct (history_at_lookup with "Hhistory_auth Hhistory_at_back") as %Hlookup.
+            iDestruct (big_sepL_lookup_acc with "Hcapacities") as "((%cap2 & Hback_estimated_capacity & _) & Hcapacities)"; first done.
+            wp_store.
+            iDestruct (front_lb_valid with "Hfront_auth Hfront_lb_front1") as %?.
+            iDestruct ("Hcapacities" with "[Hback_estimated_capacity]") as "Hcapacities"; first iSteps.
+            iSplitR "Hnew_back_next Hnew_back_data Hnew_back_index Hnew_back_estimated_capacity HΦ". { iFrameSteps. }
+            iSteps.
+
+          + iMod "HΦ" as "(%vs & (%Hvs & Hmodel₁) & _ & HΦ)".
+            iDestruct (model_agree with "Hmodel₁ Hmodel₂") as %<-.
+            iAssert ⌜
+              length vs = γ.(mpmc_bqueue_name_capacity) ∧
+              (⁺γ.(mpmc_bqueue_name_capacity) - (⁺i_back - ⁺(length past1)) = 0)%Z
+            ⌝%I as "(-> & %Hif)".
+            { iDestruct (big_sepL2_length with "Hnodes") as %?.
+              iDestruct (history_at_lookup with "Hhistory_auth Hhistory_at_back") as %?%lookup_lt_Some.
+              iPureIntro.
+              apply (f_equal length) in Hhist1. simpl_length/= in Hhist1.
+              lia.
+            }
+            rewrite bool_decide_eq_false_2; first lia.
+            iMod ("HΦ" $! false with "[$Hmodel₁ //] [//]") as "HΦ".
+
+            iSplitR "Hnew_back_next Hnew_back_data Hnew_back_index Hnew_back_estimated_capacity HΦ". { iFrameSteps. }
+            iModIntro. clear- Hif.
+
+            wp_match. do 3 wp_load. wp_pures.
+            iEval (rewrite bool_decide_eq_true_2 //).
+            iSteps.
+
+        - wp_load. do 2 wp_store. wp_pures.
+
+          wp_bind (CAS _ _ _).
+          iInv "Hinv" as "(:inv_inner =1)".
+          iDestruct (history_at_lookup with "Hhistory_auth Hhistory_at_back") as %Hlookup_back.
+          iDestruct (xtchain_lookup with "Hhist") as "(Hhist1 & _ & Hback & Hhist2)"; first done.
+          destruct (hist1 !! (S i_back)) as [next |] eqn:Hlookup_next; simpl.
+
+          + wp_cas as _ | [=].
+            iDestruct (history_at_get (S i_back) with "Hhistory_auth") as "#Hhistory_at_next"; first done.
+            iDestruct (xtchain_lookup_2 with "Hhist1 Hback_header Hback Hhist2") as "Hhist"; [done | rewrite Hlookup_next // |].
+            iSplitR "Hnew_back_next Hnew_back_data Hnew_back_index Hnew_back_estimated_capacity HΦ". { iFrameSteps. }
+            iIntros "!> {%}".
+
+            iDestruct "Hhistory_at_next" as "-#Hhistory_at_next".
+            wp_smart_apply (next_spec' back next with "[$]") as "(:node_model =next)".
+            iSteps.
+
+          + wp_cas as ? | _; first done.
+            opose proof* length_lookup_last as Hlength; [done.. |].
+            iDestruct (front_lb_valid with "Hfront_auth Hfront_lb_front") as %?.
+
+            iMod "HΦ" as "(%vs & (_ & Hmodel₁) & _ & HΦ)".
+            iDestruct (model_agree with "Hmodel₁ Hmodel₂") as %<-.
+            iMod (model_update (vs ++ [v]) with "Hmodel₁ Hmodel₂") as "(Hmodel₁ & Hmodel₂)".
+            iDestruct (big_sepL2_length with "Hnodes") as %<-.
+            assert (length nodes1 < γ.(mpmc_bqueue_name_capacity)).
+            { rewrite Hhist1 length_app /= in Hlength. lia. }
+            iEval (rewrite bool_decide_eq_true_2 //) in "HΦ".
+            iMod ("HΦ" $! true with "[$Hmodel₁ //] [//]") as "HΦ".
+
+            iDestruct (xtchain_lookup_2 with "Hhist1 Hback_header Hback []") as "Hhist"; [done | rewrite Hlookup_next // | ..].
+            { rewrite -Hlength // drop_all -xtchain_nil //. }
+            iDestruct (xtchain_snoc_2 with "Hhist Hnew_back_header Hnew_back_next") as "Hhist".
+            iDestruct (big_sepL2_snoc_2 with "Hnodes Hnew_back_data") as "Hnodes".
+            iMod (pointsto_persist with "Hnew_back_index") as "#Hnew_back_index".
+            iDestruct (big_sepL_snoc_2 new_back with "Hindices []") as "Hindices".
+            { rewrite Hlength Nat2Z.inj_succ //. }
+            iDestruct (big_sepL_snoc_2 new_back with "Hcapacities [Hnew_back_estimated_capacity]") as "Hcapacities"; first iSteps.
+            iMod (history_update new_back with "Hhistory_auth") as "(Hhistory_auth & #Hhistory_at_new_back)". rewrite Hlength.
+            iSplitR "HΦ".
+            { iFrameSteps; iPureIntro.
+              - rewrite Hhist1 -assoc //.
+              - set_solver.
+            }
+            iIntros "!> {%}".
+
+            wp_smart_apply mpmc_bqueue_fix_back_spec.
+            { iFrame "#". iSteps. }
+            iSteps.
+      }
+
+      { iClear "IHpush_2".
+
+        iIntros "%back %i_back %Φ (#Ht_capacity & #Hinv & (:node_model =back) & #Hnew_back_header & Hnew_back_next & Hnext_back_data & Hnew_back_index & Hnew_back_estimated_capacity) HΦ".
+
+        wp_rec. wp_match. wp_pures.
+
+        wp_bind (_.{estimated_capacity})%E.
+        wp_apply (wp_frame_wand with "[- HΦ]"); first iAccu.
+        iInv "Hinv" as "(:inv_inner =1)".
+        iDestruct (history_at_lookup with "Hhistory_auth Hhistory_at_back") as %Hhist1_lookup.
+        iDestruct (big_sepL_lookup_acc with "Hcapacities") as "((%cap & Hback_estimated_capacity & %Hcap) & Hcapacities)"; first done.
+        wp_load.
+        iDestruct (front_lb_get with "Hfront_auth") as "#Hfront_lb".
+        iSplitR "HΦ". { iFrameSteps. }
+        iSteps.
+      }
+    Qed.
+    #[local] Lemma mpmc_bqueue_push_2_spec t γ back i_back new_back v :
+      <<<
+        t.[capacity] ↦□ #γ.(mpmc_bqueue_name_capacity) ∗
+        inv' t γ ∗
+        node_model γ back i_back false ∗
+        new_back ↦ₕ Header §Node 4 ∗
+        new_back.[next] ↦ §Null ∗
+        new_back.[data] ↦ v ∗
+        new_back.[index] ↦- ∗
+        new_back.[estimated_capacity] ↦-
+      | ∀∀ vs,
+        ⌜length vs ≤ γ.(mpmc_bqueue_name_capacity)⌝ ∗
+        model₁ γ vs
+      >>>
+        mpmc_bqueue_push_2 #t #back #new_back @ ↑γ.(mpmc_bqueue_name_inv)
+      <<<
+        ∃∃ b,
+        ⌜b = bool_decide (length vs < γ.(mpmc_bqueue_name_capacity))⌝ ∗
+        model₁ γ (if b then vs ++ [v] else vs)
+      | RET #b;
+        True
+      >>>.
+    Proof.
+      iDestruct mpmc_bqueue_push_1_push_2_spec as "(_ & H)".
+      iApply "H".
+    Qed.
+    Lemma mpmc_bqueue_push_spec t γ ι cap v :
+      <<<
+        mpmc_bqueue_inv t γ ι cap
+      | ∀∀ vs,
+        mpmc_bqueue_model γ vs
+      >>>
+        mpmc_bqueue_push #t v @ ↑ι
+      <<<
+        ∃∃ b,
+        ⌜b = bool_decide (length vs < cap)⌝ ∗
+        mpmc_bqueue_model γ (if b then vs ++ [v] else vs)
+      | RET #b;
+        True
+      >>>.
+    Proof.
+      iIntros "%Φ (:inv) HΦ".
+
+      wp_rec.
+      wp_block new_back as "#Hnew_back_header" "_" "(Hnew_back_next & Hnew_back_data & Hnew_back_index & Hnew_back_estimated_capacity & _)".
+      wp_smart_apply (back_spec with "Hinv") as (back i_back) "(:node_model =back)".
+
+      awp_apply (mpmc_bqueue_push_2_spec with "[$]").
+      iApply (aacc_aupd_commit with "HΦ"); first done. iIntros "%vs (:model)".
+      rewrite /atomic_acc /=.
+      iStep. iSplitR; first iSteps. iIntros "!> %b (-> & $)". iSteps. iPureIntro.
+      case_bool_decide; simpl_length/=; lia.
+    Qed.
+
+    #[local] Lemma mpmc_bqueue_pop_spec_aux t γ :
+      <<<
+        inv' t γ
+      | ∀∀ vs,
+        model₁ γ vs
+      >>>
+        mpmc_bqueue_pop #t @ ↑γ.(mpmc_bqueue_name_inv)
+      <<<
+        model₁ γ (tail vs)
+      | RET head vs;
+        True
+      >>>.
+    Proof.
+      iIntros "%Φ #Hinv HΦ".
+
+      iLöb as "HLöb".
+
+      wp_rec.
+      wp_smart_apply (front_spec with "Hinv") as (front i) "(:node_model =front front=)".
+      wp_match.
+      wp_smart_apply (next_spec_pop Φ with "[$]") as (res) "[(-> & HΦ) | (%new_front & -> & (:node_model =new_front) & HΦ)]"; first iSteps.
+      wp_match. wp_pures.
+
+      wp_bind (CAS _ _ _).
+      iInv "Hinv" as "(:inv_inner =1)".
+      iDestruct (history_at_lookup with "Hhistory_auth Hhistory_at_new_front") as %Hlookup.
+      iDestruct (xtchain_lookup_acc with "Hhist") as "(_ & Hnode & Hhist)"; first done.
+      wp_cas as _ | [= <-]; first iSteps.
+      iDestruct ("Hhist" with "Hnode") as "Hhist".
+      iDestruct (history_at_lookup with "Hhistory_auth Hhistory_at_front") as %Hlookup_old.
+      iAssert ⌜length past1 = i⌝%I as %Hpast_length.
+      { iDestruct (xtchain_NoDup with "Hhist") as %Hnodup.
+        iPureIntro. eapply NoDup_lookup; try done.
+        rewrite Hhist1 list_lookup_middle //.
+      }
+      rewrite Hhist1 (assoc _ _ [_]) lookup_app_r length_app /= in Hlookup; first lia.
+      rewrite Nat.add_1_r Hpast_length Nat.sub_diag in Hlookup.
+      destruct nodes1 as [| node nodes1]; first done. injection Hlookup as ->.
+      rewrite (assoc _ _ [_]) in Hhist1.
+      iDestruct (big_sepL2_cons_inv_l with "Hnodes") as "(%v & %vs' & -> & Hfront_data & Hnodes)".
+      set past := past1 ++ [front].
+      iMod (front_update (length past) with "Hfront_auth") as "Hfront_auth".
+      { rewrite /past. simpl_length. lia. }
+      iDestruct (big_sepM_impl_thread_fupd _ (waiter_model γ past)%I with "Hwaiters Hmodel₂ [#]") as ">(Hwaiters & Hmodel₂)".
+      { iIntros "!> %waiter %j %Hlookup (%P & #Hwaiter & HP) Hmodel₂".
+        destruct (Nat.lt_trichotomy j (length past1)) as [Hj | [-> | Hj]].
+        - rewrite decide_True //.
+          rewrite /waiter_model. setoid_rewrite decide_True; last first.
+          { rewrite /past. simpl_length. lia. }
+          iSteps.
+        - rewrite decide_False; first lia.
+          rewrite /waiter_model. setoid_rewrite decide_True; last first.
+          { rewrite /past. simpl_length/=. lia. }
+          iMod "HP" as "(%vs & Hmodel₁ & _ & HP)".
+          iDestruct (model_agree with "Hmodel₁ Hmodel₂") as %->.
+          iSteps.
+        - rewrite decide_False; first lia.
+          rewrite /waiter_model. setoid_rewrite decide_False; last first.
+          { rewrite /past. simpl_length/=. lia. }
+          iSteps.
+      }
+
+      iMod "HΦ" as "(%vs & Hmodel₁ & _ & HΦ)".
+      iDestruct (model_agree with "Hmodel₁ Hmodel₂") as %->.
+      iMod (model_update vs' with "Hmodel₁ Hmodel₂") as "(Hmodel₁ & Hmodel₂)".
+      iMod ("HΦ" with "Hmodel₁") as "HΦ".
+
+      iSplitR "Hfront_data HΦ".
+      { iFrameSteps.
+        iApply (big_sepL_impl with "Hcapacities").
+        iSteps. rewrite /past length_app /=. iSteps.
+      }
+      iSteps.
+    Qed.
+    Lemma mpmc_bqueue_pop_spec t γ ι cap :
+      <<<
+        mpmc_bqueue_inv t γ ι cap
+      | ∀∀ vs,
+        mpmc_bqueue_model γ vs
+      >>>
+        mpmc_bqueue_pop #t @ ↑ι
+      <<<
+        mpmc_bqueue_model γ (tail vs)
+      | RET head vs;
+        True
+      >>>.
+    Proof.
+      iIntros "%Φ (:inv) HΦ".
+
+      wp_apply (mpmc_bqueue_pop_spec_aux with "[$]").
+      iAuIntro.
+      iApply (aacc_aupd_commit with "HΦ"); first done. iIntros "%vs (:model)".
+      iAaccIntro with "Hmodel₁"; first iSteps.
+      iStepFrameSteps. iPureIntro.
+      etrans; last done. apply length_tail.
+    Qed.
+  End mpmc_bqueue_G.
+
+  #[global] Opaque mpmc_bqueue_inv.
+  #[global] Opaque mpmc_bqueue_model.
+End base.
+
+From zoo_saturn Require
+  mpmc_bqueue__opaque.
+
 Section mpmc_bqueue_G.
   Context `{mpmc_bqueue_G : MpmcBqueueG Σ}.
 
-  Record metadata := {
-    metadata_inv : namespace ;
-    metadata_capacity : nat ;
-    metadata_history : gname ;
-    metadata_front : gname ;
-    metadata_model : gname ;
-    metadata_waiters : gname ;
-  }.
-  Implicit Types γ : metadata.
+  Implicit Types 𝑡 : location.
+  Implicit Types t : val.
 
-  #[local] Instance metadata_eq_dec : EqDecision metadata :=
-    ltac:(solve_decision).
-  #[local] Instance metadata_countable :
-    Countable metadata.
-  Proof.
-    solve_countable.
-  Qed.
-
-  #[local] Definition history_auth' γ_history :=
-    mono_list_auth γ_history (DfracOwn 1).
-  #[local] Definition history_auth γ :=
-    history_auth' γ.(metadata_history).
-  #[local] Definition history_at γ :=
-    mono_list_at γ.(metadata_history).
-
-  #[local] Definition front_auth' γ_front :=
-    auth_nat_max_auth γ_front (DfracOwn 1).
-  #[local] Definition front_auth γ :=
-    front_auth' γ.(metadata_front).
-  #[local] Definition front_lb γ :=
-    auth_nat_max_lb γ.(metadata_front).
-
-  #[local] Definition model₁' γ_model vs :=
-    twins_twin1 γ_model (DfracOwn 1) vs.
-  #[local] Definition model₁ γ :=
-    model₁' γ.(metadata_model).
-  #[local] Definition model₂' γ_model vs :=
-    twins_twin2 γ_model vs.
-  #[local] Definition model₂ γ :=
-    model₂' γ.(metadata_model).
-
-  #[local] Definition waiters_auth' γ_waiters :=
-    ghost_map_auth γ_waiters 1.
-  #[local] Definition waiters_auth γ :=
-    waiters_auth' γ.(metadata_waiters).
-  #[local] Definition waiters_at γ waiter :=
-    ghost_map_elem γ.(metadata_waiters) waiter (DfracOwn 1).
-
-  #[local] Definition node_model γ node (i : nat) b : iProp Σ :=
-    node ↦ₕ Header §Node 4 ∗
-    node.[index] ↦□ #i ∗
-    history_at γ i node ∗
-    if b then front_lb γ i else True%I.
-  #[local] Instance : CustomIpatFormat "node_model" :=
-    " ( #H{}_header &
-        #H{}_index &
-        #Hhistory_at_{} &
-        {{front}#Hfront_lb_{};_}
-      )
-    ".
-
-  #[local] Definition waiter_au γ (Ψ : bool → iProp Σ) : iProp Σ :=
-    AU <{
-      ∃∃ vs,
-      model₁ γ vs
-    }> @ ⊤ ∖ ↑γ.(metadata_inv), ∅ <{
-      model₁ γ vs
-    , COMM
-      Ψ (bool_decide (vs = []))
-    }>.
-  #[local] Definition waiter_model γ past waiter i : iProp Σ :=
-    ∃ Ψ,
-    saved_pred waiter Ψ ∗
-    if decide (i < length past) then
-      Ψ false
-    else
-      waiter_au γ Ψ.
-
-  #[local] Definition inv_inner l γ : iProp Σ :=
-    ∃ hist past front nodes back vs waiters,
-    ⌜hist = past ++ front :: nodes⌝ ∗
-    ⌜back ∈ hist⌝ ∗
-    l.[front] ↦ #front ∗
-    l.[back] ↦ #back ∗
-    xtchain (Header §Node 4) (DfracOwn 1) hist §Null ∗
-    ( [∗ list] node; v ∈ nodes; vs,
-      node.[data] ↦ v
-    ) ∗
-    ( [∗ list] i ↦ node ∈ hist,
-      node.[index] ↦□ #i
-    ) ∗
-    ( [∗ list] i ↦ node ∈ hist,
-      ∃ cap : nat,
-      node.[estimated_capacity] ↦ #cap ∗
-      ⌜i + cap ≤ length past + γ.(metadata_capacity)⌝
-    ) ∗
-    history_auth γ hist ∗
-    front_auth γ (length past) ∗
-    model₂ γ vs ∗
-    waiters_auth γ waiters ∗
-    ( [∗ map] waiter ↦ i ∈ waiters,
-      waiter_model γ past waiter i
-    ).
-  #[local] Instance : CustomIpatFormat "inv_inner" :=
-    " ( %hist{} &
-        %past{} &
-        %front{} &
-        %nodes{} &
-        %back{} &
-        %vs{} &
-        %waiters{} &
-        >%Hhist{} &
-        >%Hback{} &
-        >Hl_front &
-        >Hl_back &
-        >Hhist &
-        >Hnodes &
-        >Hindices &
-        >Hcapacities &
-        >Hhistory_auth &
-        >Hfront_auth &
-        >Hmodel₂ &
-        >Hwaiters_auth &
-        Hwaiters
-      )
-    ".
-  #[local] Definition inv' l γ :=
-    inv γ.(metadata_inv) (inv_inner l γ).
   Definition mpmc_bqueue_inv t ι cap : iProp Σ :=
-    ∃ l γ,
-    ⌜t = #l⌝ ∗
-    ⌜ι = γ.(metadata_inv)⌝ ∗
-    ⌜cap = γ.(metadata_capacity)⌝ ∗
-    meta l nroot γ ∗
-    l.[capacity] ↦□ #cap ∗
-    inv' l γ.
+    ∃ 𝑡 γ,
+    ⌜t = #𝑡⌝ ∗
+    meta 𝑡 nroot γ ∗
+    base.mpmc_bqueue_inv 𝑡 γ ι cap.
   #[local] Instance : CustomIpatFormat "inv" :=
-    " ( %l &
-        %γ &
-        -> &
-        -> &
-        -> &
-        #Hmeta &
-        #Hl_capacity &
-        #Hinv
+    " ( %𝑡{} &
+        %γ{} &
+        {%Heq{};->} &
+        #Hmeta{_{}} &
+        Hinv{_{}}
       )
     ".
 
   Definition mpmc_bqueue_model t vs : iProp Σ :=
-    ∃ l γ,
-    ⌜t = #l⌝ ∗
-    ⌜length vs ≤ γ.(metadata_capacity)⌝ ∗
-    meta l nroot γ ∗
-    model₁ γ vs.
+    ∃ 𝑡 γ,
+    ⌜t = #𝑡⌝ ∗
+    meta 𝑡 nroot γ ∗
+    base.mpmc_bqueue_model γ vs.
   #[local] Instance : CustomIpatFormat "model" :=
-    " ( %l{;_} &
-        %γ{;_} &
-        %Heq{} &
-        % &
-        #Hmeta_{} &
-        Hmodel₁{_{}}
+    " ( %𝑡{} &
+        %γ{} &
+        {%Heq{};->} &
+        Hmeta{_{}} &
+        Hmodel{_{}}
       )
     ".
 
@@ -259,154 +1379,14 @@ Section mpmc_bqueue_G.
     apply _.
   Qed.
 
-  #[local] Lemma history_alloc front :
-    ⊢ |==>
-      ∃ γ_history,
-      history_auth' γ_history [front].
-  Proof.
-    apply mono_list_alloc.
-  Qed.
-  #[local] Lemma history_at_get {γ hist} i node :
-    hist !! i = Some node →
-    history_auth γ hist ⊢
-    history_at γ i node.
-  Proof.
-    apply mono_list_at_get.
-  Qed.
-  #[local] Lemma history_at_agree γ i node1 node2 :
-    history_at γ i node1 -∗
-    history_at γ i node2 -∗
-    ⌜node1 = node2⌝.
-  Proof.
-    apply mono_list_at_agree.
-  Qed.
-  #[local] Lemma history_at_lookup γ hist i node :
-    history_auth γ hist -∗
-    history_at γ i node -∗
-    ⌜hist !! i = Some node⌝.
-  Proof.
-    apply mono_list_at_valid.
-  Qed.
-  #[local] Lemma history_at_elem_of γ hist i node :
-    history_auth γ hist -∗
-    history_at γ i node -∗
-    ⌜node ∈ hist⌝.
-  Proof.
-    iIntros "Hauth Hat".
-    iDestruct (history_at_lookup with "Hauth Hat") as %?%list_elem_of_lookup_2.
-    iSteps.
-  Qed.
-  #[local] Lemma history_update {γ hist} node :
-    history_auth γ hist ⊢ |==>
-      history_auth γ (hist ++ [node]) ∗
-      history_at γ (length hist) node.
-  Proof.
-    iIntros "Hauth".
-    iMod (mono_list_update_snoc with "Hauth") as "Hauth".
-    iDestruct (history_at_get with "Hauth") as "#Hat".
-    { rewrite lookup_snoc_Some. naive_solver. }
-    iSteps.
-  Qed.
-
-  #[local] Lemma front_alloc :
-    ⊢ |==>
-      ∃ γ_front,
-      front_auth' γ_front 0.
-  Proof.
-    apply auth_nat_max_alloc.
-  Qed.
-  #[local] Lemma front_lb_get γ i :
-    front_auth γ i ⊢
-    front_lb γ i.
-  Proof.
-    apply auth_nat_max_lb_get.
-  Qed.
-  #[local] Lemma front_lb_valid γ i1 i2 :
-    front_auth γ i1 -∗
-    front_lb γ i2 -∗
-    ⌜i2 ≤ i1⌝.
-  Proof.
-    apply auth_nat_max_lb_valid.
-  Qed.
-  #[local] Lemma front_update {γ i} i' :
-    i ≤ i' →
-    front_auth γ i ⊢ |==>
-    front_auth γ i'.
-  Proof.
-    apply auth_nat_max_update.
-  Qed.
-
-  #[local] Lemma model_alloc :
-    ⊢ |==>
-      ∃ γ_model,
-      model₁' γ_model [] ∗
-      model₂' γ_model [].
-  Proof.
-    apply twins_alloc'.
-  Qed.
-  #[local] Lemma model₁_exclusive γ vs1 vs2 :
-    model₁ γ vs1 -∗
-    model₁ γ vs2 -∗
-    False.
-  Proof.
-    apply twins_twin1_exclusive.
-  Qed.
-  #[local] Lemma model_agree γ vs1 vs2 :
-    model₁ γ vs1 -∗
-    model₂ γ vs2 -∗
-    ⌜vs1 = vs2⌝.
-  Proof.
-    apply: twins_agree_L.
-  Qed.
-  #[local] Lemma model_update {γ vs1 vs2} vs :
-    model₁ γ vs1 -∗
-    model₂ γ vs2 ==∗
-      model₁ γ vs ∗
-      model₂ γ vs.
-  Proof.
-    apply twins_update.
-  Qed.
-
-  #[local] Lemma waiters_alloc :
-    ⊢ |==>
-      ∃ γ_waiters,
-      waiters_auth' γ_waiters ∅.
-  Proof.
-    iMod ghost_map_alloc as "(%γ_waiters & Hwaiters_auth & _)".
-    iSteps.
-  Qed.
-  #[local] Lemma waiters_insert {γ waiters} i Ψ :
-    waiters_auth γ waiters ⊢ |==>
-      ∃ waiter,
-      waiters_auth γ (<[waiter := i]> waiters) ∗
-      saved_pred waiter Ψ ∗
-      waiters_at γ waiter i.
-  Proof.
-    iIntros "Hwaiters_auth".
-    iMod (saved_pred_alloc_cofinite (dom waiters) Ψ) as "(%waiter & %Hwaiter & $)".
-    rewrite not_elem_of_dom in Hwaiter.
-    iApply (ghost_map_insert with "Hwaiters_auth"); first done.
-  Qed.
-  #[local] Lemma waiters_delete γ waiters waiter i :
-    waiters_auth γ waiters -∗
-    waiters_at γ waiter i ==∗
-      ⌜waiters !! waiter = Some i⌝ ∗
-      waiters_auth γ (delete waiter waiters).
-  Proof.
-    iIntros "Hwaiters_auth Hwaiters_at".
-    iDestruct (ghost_map_lookup with "Hwaiters_auth Hwaiters_at") as %?.
-    iMod (ghost_map_delete with "Hwaiters_auth Hwaiters_at") as "$".
-    iSteps.
-  Qed.
-
   Lemma mpmc_bqueue_model_valid t ι cap vs :
     mpmc_bqueue_inv t ι cap -∗
     mpmc_bqueue_model t vs -∗
     ⌜length vs ≤ cap⌝.
   Proof.
-    iIntros "(:inv) (:model)". injection Heq as <-.
-    iDestruct (meta_agree with "Hmeta Hmeta_") as %<-. iClear "Hmeta_".
-    iSteps.
+    iIntros "(:inv =1) (:model =2)". simplify.
+    iDestruct (meta_agree with "Hmeta_1 Hmeta_2") as %->.
+    iApply (base.mpmc_bqueue_model_valid with "Hinv_1 Hmodel_2").
   Qed.
   Lemma mpmc_bqueue_model_exclusive t vs1 vs2 :
     mpmc_bqueue_model t vs1 -∗
@@ -415,7 +1395,7 @@ Section mpmc_bqueue_G.
   Proof.
     iIntros "(:model =1) (:model =2)". simplify.
     iDestruct (meta_agree with "Hmeta_1 Hmeta_2") as %->.
-    iApply (model₁_exclusive with "Hmodel₁_1 Hmodel₁_2").
+    iApply (base.mpmc_bqueue_model_exclusive with "Hmodel_1 Hmodel_2").
   Qed.
 
   Lemma mpmc_bqueue_create_spec ι cap :
@@ -432,35 +1412,10 @@ Section mpmc_bqueue_G.
   Proof.
     iIntros "%Hcap %Φ _ HΦ".
 
-    wp_rec.
-    wp_block front as "Hfront_header" "_" "(Hfront_next & Hfront_data & Hfront_index & Hfront_capacity & _)".
-    iMod (pointsto_persist with "Hfront_index") as "#Hfront_index".
-    wp_block l as "Hmeta" "(Hl_capacity & Hl_front & Hl_back & _)".
-    iMod (pointsto_persist with "Hl_capacity") as "#Hcapacity".
-
-    iMod history_alloc as "(%γ_history & Hhistory_auth)".
-    iMod front_alloc as "(%γ_front & Hfront_auth)".
-    iMod model_alloc as "(%γ_model & Hmodel₁ & Hmodel₂)".
-    iMod waiters_alloc as "(%γ_waiters & Hwaiters_auth)".
-
-    pose γ := {|
-      metadata_inv := ι ;
-      metadata_capacity := ₊cap ;
-      metadata_history := γ_history ;
-      metadata_front := γ_front ;
-      metadata_model := γ_model ;
-      metadata_waiters := γ_waiters ;
-    |}.
-
-    iMod (meta_set γ with "Hmeta") as "#Hmeta"; first done.
-
-    iApply "HΦ".
-    iSplitR "Hmodel₁"; last iSteps.
-    iExists l, γ. rewrite Z2Nat.id //. iStep 5.
-    iApply inv_alloc.
-    iExists [front], [], front, [], front, [], ∅. iFrameSteps.
-    - rewrite list_elem_of_singleton //.
-    - rewrite xtchain_singleton big_sepM_empty. iSteps.
+    iApply wp_fupd.
+    wp_apply (base.mpmc_bqueue_create_spec with "[//]") as (𝑡 γ) "(Hmeta & Hinv & Hmodel)"; first done.
+    iMod (meta_set γ with "Hmeta"); first done.
+    iSteps.
   Qed.
 
   Lemma mpmc_bqueue_capacity_spec t ι cap :
@@ -473,409 +1428,9 @@ Section mpmc_bqueue_G.
       True
     }}}.
   Proof.
-    iSteps.
-  Qed.
+    iIntros "%Φ (:inv) HΦ".
 
-  #[local] Lemma front_spec_strong Ψ l γ :
-    {{{
-      inv' l γ ∗
-      if Ψ is Some Ψ then
-        waiter_au γ Ψ
-      else
-        True
-    }}}
-      (#l).{front}
-    {{{ front i,
-      RET #front;
-      node_model γ front i true ∗
-      if Ψ is Some Ψ then
-        ∃ waiter,
-        saved_pred waiter Ψ ∗
-        waiters_at γ waiter i
-      else
-        True
-    }}}.
-  Proof.
-    iIntros "%Φ (#Hinv & HΨ) HΦ".
-
-    iInv "Hinv" as "(:inv_inner)".
-    wp_load.
-    assert (hist !! (length past) = Some front) as Hlookup.
-    { rewrite Hhist list_lookup_middle //. }
-    iDestruct (xtchain_lookup_header with "Hhist") as "#Hfront_header"; first done.
-    iDestruct (big_sepL_lookup with "Hindices") as "#Hfront_index"; first done.
-    iDestruct (history_at_get _ front with "Hhistory_auth") as "#Hhistory_at_front"; first done.
-    iDestruct (front_lb_get with "Hfront_auth") as "#Hfront_lb_front".
-    destruct Ψ as [Ψ |]; last iSteps.
-    iMod (waiters_insert (length past) Ψ with "Hwaiters_auth") as "(%waiter & Hwaiter_auth & #Hwaiter & Hwaiters_at)".
-    iDestruct (big_sepM_insert_2 _ _ waiter (length past) with "[HΨ] Hwaiters") as "Hwaiters".
-    { iExists Ψ. rewrite decide_False; first lia. iSteps. }
-    iSplitR "Hwaiters_at HΦ". { iFrameSteps. }
-    iSteps.
-  Qed.
-  #[local] Lemma front_spec l γ :
-    {{{
-      inv' l γ
-    }}}
-      (#l).{front}
-    {{{ front i,
-      RET #front;
-      node_model γ front i true
-    }}}.
-  Proof.
-    iIntros "%Φ #Hinv HΦ".
-    wp_apply (front_spec_strong None with "[$Hinv]").
-    iSteps.
-  Qed.
-
-  #[local] Lemma back_spec l γ :
-    {{{
-      inv' l γ
-    }}}
-      (#l).{back}
-    {{{ back i,
-      RET #back;
-      node_model γ back i false
-    }}}.
-  Proof.
-    iIntros "%Φ #Hinv HΦ".
-
-    iInv "Hinv" as "(:inv_inner)".
-    wp_load.
-    pose proof Hback as (i & Hlookup)%list_elem_of_lookup.
-    iDestruct (xtchain_lookup_header with "Hhist") as "#Hback_header"; first done.
-    iDestruct (big_sepL_lookup with "Hindices") as "#Hback_index"; first done.
-    iDestruct (history_at_get with "Hhistory_auth") as "#Hhistory_at_back"; first done.
-    iSplitR "HΦ". { iFrameSteps. }
-    iSteps.
-  Qed.
-
-  Inductive operation :=
-    | Size (i_front : nat) (Ψ : val → iProp Σ)
-    | IsEmpty waiter (Ψ : bool → iProp Σ)
-    | Pop (Ψ : option val → iProp Σ)
-    | Other.
-  Implicit Types op : operation.
-  Inductive operation' :=
-    | Size'
-    | IsEmpty'
-    | Pop'
-    | Other'.
-  #[local] Instance operation'_eq_dec : EqDecision operation' :=
-    ltac:(solve_decision).
-  #[local] Coercion operation_to_operation' op :=
-    match op with
-    | Size _ _ =>
-        Size'
-    | IsEmpty _ _ =>
-        IsEmpty'
-    | Pop _ =>
-        Pop'
-    | Other =>
-        Other'
-    end.
-  #[local] Definition size_au l γ Ψ : iProp Σ :=
-    AU <{
-      ∃∃ vs,
-      mpmc_bqueue_model #l vs
-    }> @ ⊤ ∖ ↑γ.(metadata_inv), ∅ <{
-      mpmc_bqueue_model #l vs
-    , COMM
-      True -∗ Ψ #(length vs)
-    }>.
-  #[local] Definition pop_au γ (Ψ : option val → iProp Σ) : iProp Σ :=
-    AU <{
-      ∃∃ vs,
-      model₁ γ vs
-    }> @ ⊤ ∖ ↑γ.(metadata_inv), ∅ <{
-      model₁ γ (tail vs)
-    , COMM
-      True -∗ Ψ (head vs)
-    }>.
-  #[local] Lemma next_spec_aux (next : option location) op l γ i node :
-    {{{
-      meta l nroot γ ∗
-      inv' l γ ∗
-      history_at γ i node ∗
-      from_option (history_at γ (S i)) True next ∗
-      match op with
-      | Size i_front Ψ =>
-          front_lb γ i_front ∗
-          size_au l γ Ψ
-      | IsEmpty waiter Ψ =>
-          front_lb γ i ∗
-          saved_pred waiter Ψ ∗
-          waiters_at γ waiter i ∗
-          £ 1
-      | Pop Ψ =>
-          front_lb γ i ∗
-          pop_au γ Ψ
-      | Other =>
-          True
-      end
-    }}}
-      (#node).{next}
-    {{{ res,
-      RET res;
-        ⌜res = §Null%V⌝ ∗
-        from_option (const False) True next ∗
-        match op with
-        | Size i_front Ψ =>
-              Ψ #(i - i_front)
-            ∨ ∃ i_front',
-              front_lb γ i_front' ∗
-              ⌜i_front < i_front'⌝ ∗
-              size_au l γ Ψ
-        | IsEmpty waiter Ψ =>
-            Ψ true
-        | Pop Ψ =>
-            Ψ None
-        | _ =>
-            True
-        end
-     ∨ ∃ node',
-        ⌜res = #node'⌝ ∗
-        node_model γ node' (S i) false ∗
-        ⌜from_option (node' =.) True next⌝ ∗
-        match op with
-        | Size _ Ψ =>
-            size_au l γ Ψ
-        | IsEmpty waiter Ψ =>
-            Ψ false
-        | Pop Ψ =>
-            pop_au γ Ψ
-        | Other =>
-            True
-        end
-    }}}.
-  Proof.
-    iIntros "%Φ (#Hmeta & #Hinv & #Hhistory_at_node & #Hhistory_at_next & Hop) HΦ".
-
-    iInv "Hinv" as "(:inv_inner)".
-    iDestruct (history_at_lookup with "Hhistory_auth Hhistory_at_node") as %Hlookup.
-    iDestruct (xtchain_lookup_acc with "Hhist") as "(_ & Hnode & Hhist)"; first done.
-    wp_load.
-    iDestruct ("Hhist" with "Hnode") as "Hhist".
-    destruct (hist !! S i) as [node' |] eqn:Hlookup'; simpl.
-
-    - iDestruct (xtchain_lookup_header with "Hhist") as "#Hnode'_header"; first done.
-      iDestruct (big_sepL_lookup with "Hindices") as "#Hnode'_index"; first done.
-      iDestruct (history_at_get (S i) with "Hhistory_auth") as "#Hhistory_at_node'"; first done.
-
-      iAssert ⌜from_option (node' =.) True next⌝%I as %?.
-      { destruct next as [next |]; last done.
-        iApply (history_at_agree with "Hhistory_at_node' Hhistory_at_next").
-      }
-
-      destruct op. 1,3,4: iSteps.
-      iDestruct "Hop" as "(#Hfront_lb_node & #Hwaiter & Hwaiters_at & H£)".
-      iMod (waiters_delete with "Hwaiters_auth Hwaiters_at") as "(%Hwaiters_lookup & Hwaiters_auth)".
-      iDestruct (big_sepM_delete with "Hwaiters") as "((%Ψ_ & Hwaiter_ & HΨ) & Hwaiters)"; first done.
-      iDestruct (saved_pred_agree false with "Hwaiter Hwaiter_") as "Heq".
-      iMod (lc_fupd_elim_later with "H£ Heq") as "Heq".
-      destruct_decide (i = length past) as -> | Hi.
-
-      + rewrite decide_False; first lia.
-
-        iMod "HΨ" as "(%vs_ & Hmodel₁ & _ & HΨ)".
-        iDestruct (model_agree with "Hmodel₁ Hmodel₂") as %->.
-        iMod ("HΨ" with "Hmodel₁") as "HΨ".
-        assert (nodes ≠ []) as Hnodes.
-        { apply lookup_lt_Some in Hlookup'.
-          rewrite Hhist length_app /= in Hlookup'.
-          naive_solver lia.
-        }
-        iAssert ⌜vs ≠ []⌝%I as %Hvs.
-        { destruct_decide (vs = []) as -> | ?; last done.
-          iDestruct (big_sepL2_length with "Hnodes") as %->%nil_length_inv.
-          iSteps.
-        }
-        rewrite bool_decide_eq_false_2 //.
-
-        iSplitR "Heq HΨ HΦ". { iFrameSteps. }
-        iSteps. iRewrite "Heq". iSteps.
-
-      + iDestruct (front_lb_valid with "Hfront_auth Hfront_lb_node") as %Hi_.
-        rewrite decide_True; first lia.
-        iSplitR "Heq HΨ HΦ". { iFrameSteps. }
-        iSteps. iRewrite "Heq". iSteps.
-
-    - destruct next as [next |].
-      { iDestruct (history_at_lookup with "Hhistory_auth Hhistory_at_next") as %?. congruence. }
-
-      destruct op as [i_front | | |].
-
-      + iDestruct "Hop" as "(#Hfront_lb_front & HΨ)".
-        destruct_decide (length past = i_front).
-
-        * iMod "HΨ" as "(%vs_ & (:model) & _ & HΨ)". injection Heq as <-.
-          iDestruct (meta_agree with "Hmeta Hmeta_") as %<-. iClear "Hmeta_".
-          iDestruct (model_agree with "Hmodel₁ Hmodel₂") as %->.
-          iMod ("HΨ" with "[Hmodel₁] [//]") as "HΨ"; first iSteps.
-          assert ((i - i_front)%Z = length nodes) as ->.
-          { opose proof* length_lookup_last as Hlength; [done.. |].
-            rewrite Hhist length_app /= in Hlength.
-            lia.
-          }
-          iDestruct (big_sepL2_length with "Hnodes") as %->.
-
-          iSplitR "HΨ HΦ". { iFrameSteps. }
-          iSteps.
-
-        * iDestruct (front_lb_valid with "Hfront_auth Hfront_lb_front") as %?. iClear "Hfront_lb_front".
-          iDestruct (front_lb_get with "Hfront_auth") as "#Hfront_lb_front".
-          iSplitR "HΨ HΦ". { iFrameSteps. }
-          iSteps.
-
-      + iDestruct "Hop" as "(#Hfront_lb_node & #Hwaiter & Hwaiters_at & H£)".
-        iDestruct (front_lb_valid with "Hfront_auth Hfront_lb_node") as %Hi.
-        opose proof* length_lookup_last as Hlength; [done.. |].
-        rewrite Hhist length_app /= in Hlength.
-        assert (i = length past) as -> by lia.
-        assert (length nodes = 0) as ->%nil_length_inv by lia.
-        iDestruct (big_sepL2_length with "Hnodes") as %->%symmetry%nil_length_inv.
-        iMod (waiters_delete with "Hwaiters_auth Hwaiters_at") as "(%Hwaiters_lookup & Hwaiters_auth)".
-        iDestruct (big_sepM_delete with "Hwaiters") as "((%Ψ_ & Hwaiter_ & HΨ) & Hwaiters)"; first done.
-        iDestruct (saved_pred_agree true with "Hwaiter Hwaiter_") as "Heq".
-        iMod (lc_fupd_elim_later with "H£ Heq") as "Heq".
-        rewrite decide_False; first lia.
-
-        iMod "HΨ" as "(%vs & Hmodel₁ & _ & HΨ)".
-        iDestruct (model_agree with "Hmodel₁ Hmodel₂") as %->.
-        iMod ("HΨ" with "Hmodel₁") as "HΨ".
-
-        iSplitR "Heq HΨ HΦ". { iFrameSteps. }
-        iIntros "!> {%}".
-
-        iApply "HΦ".
-        iLeft. iRewrite "Heq". iSteps.
-
-      + iDestruct "Hop" as "(#Hfront_lb_node & HΨ)".
-        iDestruct (front_lb_valid with "Hfront_auth Hfront_lb_node") as %Hi.
-        opose proof* length_lookup_last as Hlength; [done.. |].
-        rewrite Hhist length_app /= in Hlength.
-        assert (i = length past) as -> by lia.
-        assert (length nodes = 0) as ->%nil_length_inv by lia.
-        iDestruct (big_sepL2_length with "Hnodes") as %->%symmetry%nil_length_inv.
-
-        iMod "HΨ" as "(%vs & Hmodel₁ & _ & HΨ)".
-        iDestruct (model_agree with "Hmodel₁ Hmodel₂") as %->.
-        iMod ("HΨ" with "Hmodel₁") as "HΨ".
-
-        iSplitR "HΨ HΦ". { iFrameSteps. }
-        iSteps.
-
-      + iSteps.
-  Qed.
-  #[local] Lemma next_spec {l γ i} node :
-    {{{
-      meta l nroot γ ∗
-      inv' l γ ∗
-      history_at γ i node
-    }}}
-      (#node).{next}
-    {{{ res,
-      RET res;
-        ⌜res = §Null%V⌝
-      ∨ ∃ node',
-        ⌜res = #node'⌝ ∗
-        node_model γ node' (S i) false
-    }}}.
-  Proof.
-    iIntros "%Φ (#Hmeta & #Hinv & #Hhistory_at_node) HΦ".
-    wp_apply (next_spec_aux None Other); iSteps.
-  Qed.
-  #[local] Lemma next_spec' {l γ i} node next :
-    {{{
-      meta l nroot γ ∗
-      inv' l γ ∗
-      history_at γ i node ∗
-      history_at γ (S i) next
-    }}}
-      (#node).{next}
-    {{{
-      RET #next;
-      node_model γ next (S i) false
-    }}}.
-  Proof.
-    iIntros "%Φ (#Hmeta & #Hinv & #Hhistory_at_node & #Hhistory_at_next) HΦ".
-    wp_apply (next_spec_aux (Some next) Other); iSteps.
-  Qed.
-  #[local] Lemma next_spec_size {l γ i node} i_front Ψ :
-    {{{
-      meta l nroot γ ∗
-      inv' l γ ∗
-      history_at γ i node ∗
-      front_lb γ i_front ∗
-      size_au l γ Ψ
-    }}}
-      (#node).{next}
-    {{{ res,
-      RET res;
-        ⌜res = §Null%V⌝ ∗
-        ( Ψ #(i - i_front)
-        ∨ ∃ i_front',
-          front_lb γ i_front' ∗
-          ⌜i_front < i_front'⌝ ∗
-          size_au l γ Ψ
-        )
-     ∨ ∃ node',
-        ⌜res = #node'⌝ ∗
-        node_model γ node' (S i) false ∗
-        size_au l γ Ψ
-    }}}.
-  Proof.
-    iIntros "%Φ (#Hmeta & #Hinv & #Hhistory_at_node & #Hfront_lb_front & HΨ) HΦ".
-    wp_apply (next_spec_aux None (Size _ _) with "[$]").
-    iSteps.
-  Qed.
-  #[local] Lemma next_spec_is_empty {l γ i node} waiter Ψ :
-    {{{
-      meta l nroot γ ∗
-      inv' l γ ∗
-      history_at γ i node ∗
-      front_lb γ i ∗
-      saved_pred waiter Ψ ∗
-      waiters_at γ waiter i ∗
-      £ 1
-    }}}
-      (#node).{next}
-    {{{ res,
-      RET res;
-        ⌜res = §Null%V⌝ ∗
-        Ψ true
-      ∨ ∃ node',
-        ⌜res = #node'⌝ ∗
-        node_model γ node' (S i) false ∗
-        Ψ false
-    }}}.
-  Proof.
-    iIntros "%Φ (#Hmeta & #Hinv & #Hhistory_at_node & #Hfront_lb_node & #Hwaiter & Hwaiters_at & H£) HΦ".
-    wp_apply (next_spec_aux None (IsEmpty _ _) with "[$]").
-    iSteps.
-  Qed.
-  #[local] Lemma next_spec_pop {l γ i node} Ψ :
-    {{{
-      meta l nroot γ ∗
-      inv' l γ ∗
-      history_at γ i node ∗
-      front_lb γ i ∗
-      pop_au γ Ψ
-    }}}
-      (#node).{next}
-    {{{ res,
-      RET res;
-        ⌜res = §Null%V⌝ ∗
-        Ψ None
-      ∨ ∃ node',
-        ⌜res = #node'⌝ ∗
-        node_model γ node' (S i) false ∗
-        pop_au γ Ψ
-    }}}.
-  Proof.
-    iIntros "%Φ (#Hmeta & #Hinv & #Hhistory_at_node & #Hfront_lb_node & HΨ) HΦ".
-    wp_apply (next_spec_aux None (Pop _) with "[$]").
-    iSteps.
+    wp_apply (base.mpmc_bqueue_capacity_spec with "[$] HΦ").
   Qed.
 
   Lemma mpmc_bqueue_size_spec t ι cap :
@@ -893,65 +1448,11 @@ Section mpmc_bqueue_G.
   Proof.
     iIntros "%Φ (:inv) HΦ".
 
-    iLöb as "HLöb".
-
-    wp_rec.
-    wp_apply (front_spec with "Hinv") as (front1 i_front1) "(:node_model =front1 front=)".
-    wp_match.
-    wp_smart_apply (prophet_typed_strong_1_wp_proph prophet with "[//]") as (pid proph) "Hproph".
-    wp_smart_apply (back_spec with "Hinv") as (back2 i_back2) "(:node_model =back2)".
-    wp_match. wp_pures.
-    destruct_decide (proph = front1) as -> | Hproph.
-
-    - wp_apply (next_spec_size with "[$]") as (res) "[(-> & HΦ) | (%node & -> & (:node_model =node) & HΦ)]".
-
-      + wp_pures.
-
-        wp_bind (Resolve _ _ _).
-        iInv "Hinv" as "(:inv_inner =3)".
-        wp_apply (prophet_typed_strong_1_wp_resolve with "Hproph"); first done.
-        wp_load.
-        iStep. iIntros "<-".
-        iDestruct "HΦ" as "[HΦ | (%i_front2 & #Hfront_lb_front2 & % & HΦ)]"; last first.
-        { assert (hist3 !! (length past3) = Some front1) as Hlookup.
-          { rewrite Hhist3 list_lookup_middle //. }
-          iDestruct (big_sepL_lookup with "Hindices") as "#Hfront1_index_"; first done.
-          iDestruct (pointsto_agree with "Hfront1_index Hfront1_index_") as %[= ?%(inj _)].
-          iDestruct (front_lb_valid with "Hfront_auth Hfront_lb_front2") as %?.
-          lia.
-        }
-        iSteps.
-
-      + wp_match. wp_pures.
-
-        wp_bind (CAS _ _ _).
-        iInv "Hinv" as "(:inv_inner =3)".
-        wp_apply (wp_cas_nobranch' with "Hl_back") as (b) "% Hl_back".
-        iSplitR "HΦ".
-        { iDestruct (history_at_elem_of with "Hhistory_auth Hhistory_at_node") as %Hnode.
-          destruct b; iFrameSteps.
-        }
-        iSteps.
-
-    - wp_apply (next_spec with "[$]") as (res) "[-> | (%node & -> & (:node_model =node))]".
-
-      + wp_pures.
-
-        wp_bind (Resolve _ _ _).
-        iInv "Hinv" as "(:inv_inner =3)".
-        wp_apply (prophet_typed_strong_1_wp_resolve with "Hproph"); first done.
-        iSteps.
-
-      + wp_match. wp_pures.
-
-        wp_bind (CAS _ _ _).
-        iInv "Hinv" as "(:inv_inner =3)".
-        wp_apply (wp_cas_nobranch' with "Hl_back") as (b) "% Hl_back".
-        iSplitR "HΦ".
-        { iDestruct (history_at_elem_of with "Hhistory_auth Hhistory_at_node") as %Hnode.
-          destruct b; iFrameSteps.
-        }
-        iSteps.
+    awp_apply (base.mpmc_bqueue_size_spec with "[$]").
+    { iApply (aacc_aupd_commit with "HΦ"); first done. iIntros "%vs (:model =1)". simplify.
+      iDestruct (meta_agree with "Hmeta Hmeta_1") as %<-. iClear "Hmeta_1".
+      iAaccIntro with "Hmodel_1"; iSteps.
+    }
   Qed.
 
   Lemma mpmc_bqueue_is_empty_spec t ι cap :
@@ -969,264 +1470,13 @@ Section mpmc_bqueue_G.
   Proof.
     iIntros "%Φ (:inv) HΦ".
 
-    wp_rec credit:"H£".
-    wp_smart_apply (front_spec_strong (Some $ λ b, Φ #b) with "[$Hinv HΦ]") as (node i) "((:node_model =node front=) & %waiter & #Hwaiter & Hwaiters_at)".
-    { rewrite /= /waiter_au. iAuIntro.
-      iApply (aacc_aupd_commit with "HΦ"); first done. iIntros "%vs (:model)". injection Heq as <-.
-      iDestruct (meta_agree with "Hmeta Hmeta_") as %<-. iClear "Hmeta_".
-      iAaccIntro with "Hmodel₁"; iSteps.
-    }
-    wp_match.
-    wp_smart_apply (next_spec_is_empty with "[$]"); iSteps.
-  Qed.
-
-  #[local] Lemma mpmc_bqueue_fix_back_spec {l γ} i {back} j new_back :
-    {{{
-      meta l nroot γ ∗
-      inv' l γ ∗
-      history_at γ i back ∗
-      node_model γ new_back j false
-    }}}
-      mpmc_bqueue_fix_back #l #back #new_back
-    {{{
-      RET ();
-      True
-    }}}.
-  Proof.
-    iIntros "%Φ (#Hmeta & #Hinv & #Hhistory_at_back & (:node_model =new_back)) HΦ".
-
-    iLöb as "HLöb" forall (i back) "Hhistory_at_back".
-
-    wp_rec. wp_match.
-
-    wp_bind (_ and _)%E.
-    wp_apply (wp_wand itype_bool) as (res) "(%b & ->)".
-    { wp_smart_apply (next_spec new_back with "[$]") as (res) "[-> | (%new_back' & -> & (:node_model =new_back'))]"; last iSteps.
-      wp_pures.
-
-      wp_bind (CAS _ _ _).
-      iInv "Hinv" as "(:inv_inner =1)".
-      wp_cas as _ | [= ->]; first iSteps.
-      iDestruct (history_at_lookup with "Hhistory_auth Hhistory_at_new_back") as %Hnew_back%list_elem_of_lookup_2.
-      iSteps.
-    }
-
-    destruct b; last iSteps.
-    wp_smart_apply domain_yield_spec.
-    wp_smart_apply (back_spec with "Hinv") as (back' i') "(:node_model =back')".
-    iApply ("HLöb" with "HΦ Hhistory_at_back'").
-  Qed.
-
-  #[local] Lemma mpmc_bqueue_push_1_push_2_spec l γ new_back v :
-    ⊢ (
-      ∀ back i_back i_front (cap : Z),
-      <<<
-        meta l nroot γ ∗
-        l.[capacity] ↦□ #γ.(metadata_capacity) ∗
-        inv' l γ ∗
-        node_model γ back i_back false ∗
-        front_lb γ i_front ∗
-        ⌜0 ≤ cap⌝%Z ∗
-        ⌜i_back + cap ≤ i_front + γ.(metadata_capacity)⌝%Z ∗
-        new_back ↦ₕ Header §Node 4 ∗
-        new_back.[next] ↦ §Null ∗
-        new_back.[data] ↦ v ∗
-        new_back.[index] ↦- ∗
-        new_back.[estimated_capacity] ↦-
-      | ∀∀ vs,
-        ⌜length vs ≤ γ.(metadata_capacity)⌝ ∗
-        model₁ γ vs
-      >>>
-        mpmc_bqueue_push_1 #l #back #cap #new_back @ ↑γ.(metadata_inv)
-      <<<
-        ∃∃ b,
-        ⌜b = bool_decide (length vs < γ.(metadata_capacity))⌝ ∗
-        model₁ γ (if b then vs ++ [v] else vs)
-      | RET #b;
-        True
-      >>>
-    ) ∧ (
-      ∀ back i_back,
-      <<<
-        meta l nroot γ ∗
-        l.[capacity] ↦□ #γ.(metadata_capacity) ∗
-        inv' l γ ∗
-        node_model γ back i_back false ∗
-        new_back ↦ₕ Header §Node 4 ∗
-        new_back.[next] ↦ §Null ∗
-        new_back.[data] ↦ v ∗
-        new_back.[index] ↦- ∗
-        new_back.[estimated_capacity] ↦-
-      | ∀∀ vs,
-        ⌜length vs ≤ γ.(metadata_capacity)⌝ ∗
-        model₁ γ vs
-      >>>
-        mpmc_bqueue_push_2 #l #back #new_back @ ↑γ.(metadata_inv)
-      <<<
-        ∃∃ b,
-        ⌜b = bool_decide (length vs < γ.(metadata_capacity))⌝ ∗
-        model₁ γ (if b then vs ++ [v] else vs)
-      | RET #b;
-        True
-      >>>
-    ).
-  Proof.
-    iLöb as "HLöb".
-    iDestruct "HLöb" as "(IHpush_1 & IHpush_2)".
-    iSplit.
-
-    { iIntros "%back %i_back %i_front %cap %Φ (#Hmeta & #Hl_capacity & #Hinv & (:node_model =back) & #Hfront_lb_front & % & % & #Hnew_back_header & Hnew_back_next & Hnew_back_data & (% & Hnew_back_index) & (% & Hnew_back_estimated_capacity)) HΦ".
-
-      wp_rec. do 2 wp_match. wp_pures.
-      case_bool_decide; wp_pures.
-
-      - wp_bind (_.{front})%E.
-        iInv "Hinv" as "(:inv_inner =1)".
-        wp_load.
-        assert (hist1 !! (length past1) = Some front1) as Hlookup.
-        { rewrite Hhist1 list_lookup_middle //. }
-        iDestruct (xtchain_lookup_header with "Hhist") as "#Hfront1_header"; first done.
-        iDestruct (big_sepL_lookup with "Hindices") as "#Hfront1_index"; first done.
-
-        destruct_decide (i_back < length past1 + γ.(metadata_capacity)) as Hnotfull | Hfull.
-
-        + iDestruct (front_lb_get with "Hfront_auth") as "#Hfront_lb_front1".
-          iSplitR "Hnew_back_next Hnew_back_data Hnew_back_index Hnew_back_estimated_capacity HΦ". { iFrameSteps. }
-          remember (length past1) as i_front1.
-          iModIntro. clear- Hnotfull.
-
-          wp_match. do 3 wp_load. wp_pures.
-          rewrite bool_decide_eq_false_2; first lia.
-          wp_pures.
-
-          wp_bind (_ <-{estimated_capacity} _)%E.
-          iInv "Hinv" as "(:inv_inner =2)".
-          iDestruct (history_at_lookup with "Hhistory_auth Hhistory_at_back") as %Hlookup.
-          iDestruct (big_sepL_lookup_acc with "Hcapacities") as "((%cap2 & Hback_estimated_capacity & _) & Hcapacities)"; first done.
-          wp_store.
-          iDestruct (front_lb_valid with "Hfront_auth Hfront_lb_front1") as %?.
-          iDestruct ("Hcapacities" with "[Hback_estimated_capacity]") as "Hcapacities"; first iSteps.
-          iSplitR "Hnew_back_next Hnew_back_data Hnew_back_index Hnew_back_estimated_capacity HΦ". { iFrameSteps. }
-          iSteps.
-
-        + iMod "HΦ" as "(%vs & (%Hvs & Hmodel₁) & _ & HΦ)".
-          iDestruct (model_agree with "Hmodel₁ Hmodel₂") as %<-.
-          iAssert ⌜
-            length vs = γ.(metadata_capacity) ∧
-            (⁺γ.(metadata_capacity) - (⁺i_back - ⁺(length past1)) = 0)%Z
-          ⌝%I as "(-> & %Hif)".
-          { iDestruct (big_sepL2_length with "Hnodes") as %?.
-            iDestruct (history_at_lookup with "Hhistory_auth Hhistory_at_back") as %?%lookup_lt_Some.
-            iPureIntro.
-            apply (f_equal length) in Hhist1. simpl_length/= in Hhist1.
-            lia.
-          }
-          rewrite bool_decide_eq_false_2; first lia.
-          iMod ("HΦ" $! false with "[$Hmodel₁ //] [//]") as "HΦ".
-
-          iSplitR "Hnew_back_next Hnew_back_data Hnew_back_index Hnew_back_estimated_capacity HΦ". { iFrameSteps. }
-          iModIntro. clear- Hif.
-
-          wp_match. do 3 wp_load. wp_pures.
-          iEval (rewrite bool_decide_eq_true_2 //).
-          iSteps.
-
-      - wp_load. do 2 wp_store. wp_pures.
-
-        wp_bind (CAS _ _ _).
-        iInv "Hinv" as "(:inv_inner =1)".
-        iDestruct (history_at_lookup with "Hhistory_auth Hhistory_at_back") as %Hlookup_back.
-        iDestruct (xtchain_lookup with "Hhist") as "(Hhist1 & _ & Hback & Hhist2)"; first done.
-        destruct (hist1 !! (S i_back)) as [next |] eqn:Hlookup_next; simpl.
-
-        + wp_cas as _ | [=].
-          iDestruct (history_at_get (S i_back) with "Hhistory_auth") as "#Hhistory_at_next"; first done.
-          iDestruct (xtchain_lookup_2 with "Hhist1 Hback_header Hback Hhist2") as "Hhist"; [done | rewrite Hlookup_next // |].
-          iSplitR "Hnew_back_next Hnew_back_data Hnew_back_index Hnew_back_estimated_capacity HΦ". { iFrameSteps. }
-          iIntros "!> {%}".
-
-          iDestruct "Hhistory_at_next" as "-#Hhistory_at_next".
-          wp_smart_apply (next_spec' back next with "[$]") as "(:node_model =next)".
-          iSteps.
-
-        + wp_cas as ? | _; first done.
-          opose proof* length_lookup_last as Hlength; [done.. |].
-          iDestruct (front_lb_valid with "Hfront_auth Hfront_lb_front") as %?.
-
-          iMod "HΦ" as "(%vs & (_ & Hmodel₁) & _ & HΦ)".
-          iDestruct (model_agree with "Hmodel₁ Hmodel₂") as %<-.
-          iMod (model_update (vs ++ [v]) with "Hmodel₁ Hmodel₂") as "(Hmodel₁ & Hmodel₂)".
-          iDestruct (big_sepL2_length with "Hnodes") as %<-.
-          assert (length nodes1 < γ.(metadata_capacity)).
-          { rewrite Hhist1 length_app /= in Hlength. lia. }
-          iEval (rewrite bool_decide_eq_true_2 //) in "HΦ".
-          iMod ("HΦ" $! true with "[$Hmodel₁ //] [//]") as "HΦ".
-
-          iDestruct (xtchain_lookup_2 with "Hhist1 Hback_header Hback []") as "Hhist"; [done | rewrite Hlookup_next // | ..].
-          { rewrite -Hlength // drop_all -xtchain_nil //. }
-          iDestruct (xtchain_snoc_2 with "Hhist Hnew_back_header Hnew_back_next") as "Hhist".
-          iDestruct (big_sepL2_snoc_2 with "Hnodes Hnew_back_data") as "Hnodes".
-          iMod (pointsto_persist with "Hnew_back_index") as "#Hnew_back_index".
-          iDestruct (big_sepL_snoc_2 new_back with "Hindices []") as "Hindices".
-          { rewrite Hlength Nat2Z.inj_succ //. }
-          iDestruct (big_sepL_snoc_2 new_back with "Hcapacities [Hnew_back_estimated_capacity]") as "Hcapacities"; first iSteps.
-          iMod (history_update new_back with "Hhistory_auth") as "(Hhistory_auth & #Hhistory_at_new_back)". rewrite Hlength.
-          iSplitR "HΦ".
-          { iFrameSteps; iPureIntro.
-            - rewrite Hhist1 -assoc //.
-            - set_solver.
-          }
-          iIntros "!> {%}".
-
-          wp_smart_apply mpmc_bqueue_fix_back_spec.
-          { iFrame "#". iSteps. }
-          iSteps.
-    }
-
-    { iClear "IHpush_2".
-
-      iIntros "%back %i_back %Φ (#Hmeta & #Hl_capacity & #Hinv & (:node_model =back) & #Hnew_back_header & Hnew_back_next & Hnext_back_data & Hnew_back_index & Hnew_back_estimated_capacity) HΦ".
-
-      wp_rec. wp_match. wp_pures.
-
-      wp_bind (_.{estimated_capacity})%E.
-      wp_apply (wp_frame_wand with "[- HΦ]"); first iAccu.
-      iInv "Hinv" as "(:inv_inner =1)".
-      iDestruct (history_at_lookup with "Hhistory_auth Hhistory_at_back") as %Hhist1_lookup.
-      iDestruct (big_sepL_lookup_acc with "Hcapacities") as "((%cap & Hback_estimated_capacity & %Hcap) & Hcapacities)"; first done.
-      wp_load.
-      iDestruct (front_lb_get with "Hfront_auth") as "#Hfront_lb".
-      iSplitR "HΦ". { iFrameSteps. }
-      iSteps.
+    awp_apply (base.mpmc_bqueue_is_empty_spec with "[$]").
+    { iApply (aacc_aupd_commit with "HΦ"); first done. iIntros "%vs (:model =1)". simplify.
+      iDestruct (meta_agree with "Hmeta Hmeta_1") as %<-. iClear "Hmeta_1".
+      iAaccIntro with "Hmodel_1"; iSteps.
     }
   Qed.
-  #[local] Lemma mpmc_bqueue_push_2_spec l γ back i_back new_back v :
-    <<<
-      meta l nroot γ ∗
-      l.[capacity] ↦□ #γ.(metadata_capacity) ∗
-      inv' l γ ∗
-      node_model γ back i_back false ∗
-      new_back ↦ₕ Header §Node 4 ∗
-      new_back.[next] ↦ §Null ∗
-      new_back.[data] ↦ v ∗
-      new_back.[index] ↦- ∗
-      new_back.[estimated_capacity] ↦-
-    | ∀∀ vs,
-      ⌜length vs ≤ γ.(metadata_capacity)⌝ ∗
-      model₁ γ vs
-    >>>
-      mpmc_bqueue_push_2 #l #back #new_back @ ↑γ.(metadata_inv)
-    <<<
-      ∃∃ b,
-      ⌜b = bool_decide (length vs < γ.(metadata_capacity))⌝ ∗
-      model₁ γ (if b then vs ++ [v] else vs)
-    | RET #b;
-      True
-    >>>.
-  Proof.
-    iDestruct mpmc_bqueue_push_1_push_2_spec as "(_ & H)".
-    iApply "H".
-  Qed.
+
   Lemma mpmc_bqueue_push_spec t ι cap v :
     <<<
       mpmc_bqueue_inv t ι cap
@@ -1244,93 +1494,13 @@ Section mpmc_bqueue_G.
   Proof.
     iIntros "%Φ (:inv) HΦ".
 
-    wp_rec.
-    wp_block new_back as "#Hnew_back_header" "_" "(Hnew_back_next & Hnew_back_data & Hnew_back_index & Hnew_back_estimated_capacity & _)".
-    wp_smart_apply (back_spec with "Hinv") as (back i_back) "(:node_model =back)".
-
-    awp_apply (mpmc_bqueue_push_2_spec with "[$]").
-    iApply (aacc_aupd_commit with "HΦ"); first done. iIntros "%vs (:model)". injection Heq as <-.
-    iDestruct (meta_agree with "Hmeta Hmeta_") as %<-. iClear "Hmeta_".
-    rewrite /atomic_acc /=.
-    iStep. iSplitR; first iSteps. iIntros "!> %b (-> & $)". iSteps. iPureIntro.
-    case_bool_decide; simpl_length/=; lia.
+    awp_apply (base.mpmc_bqueue_push_spec with "[$]").
+    { iApply (aacc_aupd_commit with "HΦ"); first done. iIntros "%vs (:model =1)". simplify.
+      iDestruct (meta_agree with "Hmeta Hmeta_1") as %<-. iClear "Hmeta_1".
+      iAaccIntro with "Hmodel_1"; iSteps.
+    }
   Qed.
 
-  #[local] Lemma mpmc_bqueue_pop_spec_aux l γ :
-    <<<
-      meta l nroot γ ∗
-      inv' l γ
-    | ∀∀ vs,
-      model₁ γ vs
-    >>>
-      mpmc_bqueue_pop #l @ ↑γ.(metadata_inv)
-    <<<
-      model₁ γ (tail vs)
-    | RET head vs;
-      True
-    >>>.
-  Proof.
-    iIntros "%Φ (#Hmeta & #Hinv) HΦ".
-
-    iLöb as "HLöb".
-
-    wp_rec.
-    wp_smart_apply (front_spec with "Hinv") as (front i) "(:node_model =front front=)".
-    wp_match.
-    wp_smart_apply (next_spec_pop Φ with "[$]") as (res) "[(-> & HΦ) | (%new_front & -> & (:node_model =new_front) & HΦ)]"; first iSteps.
-    wp_match. wp_pures.
-
-    wp_bind (CAS _ _ _).
-    iInv "Hinv" as "(:inv_inner =1)".
-    iDestruct (history_at_lookup with "Hhistory_auth Hhistory_at_new_front") as %Hlookup.
-    iDestruct (xtchain_lookup_acc with "Hhist") as "(_ & Hnode & Hhist)"; first done.
-    wp_cas as _ | [= <-]; first iSteps.
-    iDestruct ("Hhist" with "Hnode") as "Hhist".
-    iDestruct (history_at_lookup with "Hhistory_auth Hhistory_at_front") as %Hlookup_old.
-    iAssert ⌜length past1 = i⌝%I as %Hpast_length.
-    { iDestruct (xtchain_NoDup with "Hhist") as %Hnodup.
-      iPureIntro. eapply NoDup_lookup; try done.
-      rewrite Hhist1 list_lookup_middle //.
-    }
-    rewrite Hhist1 (assoc _ _ [_]) lookup_app_r length_app /= in Hlookup; first lia.
-    rewrite Nat.add_1_r Hpast_length Nat.sub_diag in Hlookup.
-    destruct nodes1 as [| node nodes1]; first done. injection Hlookup as ->.
-    rewrite (assoc _ _ [_]) in Hhist1.
-    iDestruct (big_sepL2_cons_inv_l with "Hnodes") as "(%v & %vs' & -> & Hfront_data & Hnodes)".
-    set past := past1 ++ [front].
-    iMod (front_update (length past) with "Hfront_auth") as "Hfront_auth".
-    { rewrite /past. simpl_length. lia. }
-    iDestruct (big_sepM_impl_thread_fupd _ (waiter_model γ past)%I with "Hwaiters Hmodel₂ [#]") as ">(Hwaiters & Hmodel₂)".
-    { iIntros "!> %waiter %j %Hlookup (%P & #Hwaiter & HP) Hmodel₂".
-      destruct (Nat.lt_trichotomy j (length past1)) as [Hj | [-> | Hj]].
-      - rewrite decide_True //.
-        rewrite /waiter_model. setoid_rewrite decide_True; last first.
-        { rewrite /past. simpl_length. lia. }
-        iSteps.
-      - rewrite decide_False; first lia.
-        rewrite /waiter_model. setoid_rewrite decide_True; last first.
-        { rewrite /past. simpl_length/=. lia. }
-        iMod "HP" as "(%vs & Hmodel₁ & _ & HP)".
-        iDestruct (model_agree with "Hmodel₁ Hmodel₂") as %->.
-        iSteps.
-      - rewrite decide_False; first lia.
-        rewrite /waiter_model. setoid_rewrite decide_False; last first.
-        { rewrite /past. simpl_length/=. lia. }
-        iSteps.
-    }
-
-    iMod "HΦ" as "(%vs & Hmodel₁ & _ & HΦ)".
-    iDestruct (model_agree with "Hmodel₁ Hmodel₂") as %->.
-    iMod (model_update vs' with "Hmodel₁ Hmodel₂") as "(Hmodel₁ & Hmodel₂)".
-    iMod ("HΦ" with "Hmodel₁") as "HΦ".
-
-    iSplitR "Hfront_data HΦ".
-    { iFrameSteps.
-      iApply (big_sepL_impl with "Hcapacities").
-      iSteps. rewrite /past length_app /=. iSteps.
-    }
-    iSteps.
-  Qed.
   Lemma mpmc_bqueue_pop_spec t ι cap :
     <<<
       mpmc_bqueue_inv t ι cap
@@ -1346,18 +1516,13 @@ Section mpmc_bqueue_G.
   Proof.
     iIntros "%Φ (:inv) HΦ".
 
-    wp_apply (mpmc_bqueue_pop_spec_aux with "[$]").
-    iAuIntro.
-    iApply (aacc_aupd_commit with "HΦ"); first done. iIntros "%vs (:model)". injection Heq as <-.
-    iDestruct (meta_agree with "Hmeta Hmeta_") as %<-.
-    iAaccIntro with "Hmodel₁"; first iSteps.
-    iStepFrameSteps. iPureIntro.
-    etrans; last done. apply length_tail.
+    awp_apply (base.mpmc_bqueue_pop_spec with "[$]").
+    { iApply (aacc_aupd_commit with "HΦ"); first done. iIntros "%vs (:model =1)". simplify.
+      iDestruct (meta_agree with "Hmeta Hmeta_1") as %<-. iClear "Hmeta_1".
+      iAaccIntro with "Hmodel_1"; iSteps.
+    }
   Qed.
 End mpmc_bqueue_G.
-
-From zoo_saturn Require
-  mpmc_bqueue__opaque.
 
 #[global] Opaque mpmc_bqueue_inv.
 #[global] Opaque mpmc_bqueue_model.
